on progresse vers le niveau 4
git-svn-id: svn+ssh://cplex.ensiie.fr/home/julien.forest/svnpub/ill_coq@90 c0685fd8-6de5-4121-bad2-4297bca5a80f

emma.v
@@ -361,775 +361,3543 @@ Proof with try solve [ apply Id;reflexivity | prove_multiset_eq].
   weak_impl_l V A...
   apply Oplus_R_1...
 Qed.
+
+(*
+Notation "'all_proofs_of' x" := (forall (p:x), exists_AtheseA_on_formula (fun _ _ _ => trueP) A M _ _ p =trueP) (at level 80,only parsing).
+
+Notation "'no_proof_for' x" := (forall (p:x), False) (at level 80,only parsing).
+*)
+
+Definition all_proofs_of env gamma := (forall (p:env⊢gamma), exists_AtheseA_on_formula (fun _ _ _ => trueP) A M _ _ p =trueP).
+
+Definition no_proof_for env gamma := (forall (p:env⊢gamma), False).
+Hint Unfold all_proofs_of no_proof_for : proof.
+
+Lemma all_proofs_of_pre_morph : forall φ Γ Γ',  
+  all_proofs_of Γ φ -> eq_bool Γ Γ' = true -> all_proofs_of Γ' φ.
+Proof.
+  unfold all_proofs_of.
+  intros φ Γ Γ' Hall Heq p.
+  apply eq_bool_correct in Heq.
+  assert (h:exists p': Γ⊢φ, Proof_eq.eq p p').
+    symmetry in Heq; exists (ILL_proof_pre_morph _ _ _ Heq p).
+    apply Proof_eq.sym;apply Proof_eq.eq_pre_morph.
+      destruct h as [p' h].
+      rewrite exists_AtheseA_on_formula_proof_eq_compat with (h2:=p') (1:=h); auto.
+Qed.
+Hint Resolve all_proofs_of_pre_morph : proof.
+
+
+Lemma all_proofs_of_pre_morph' : 
+  forall φ Γ Γ', all_proofs_of Γ φ -> eq_bool Γ Γ' = true -> 
+    forall (p:Γ'⊢φ), exists_AtheseA_on_formula (fun _ _ _ => trueP) A M _ _ p =trueP.
+Proof.
+  intros φ Γ Γ' H H0 p.  
+  eapply all_proofs_of_pre_morph;eassumption.
+Qed.
+Hint Resolve all_proofs_of_pre_morph' : proof.
+Hint Rewrite all_proofs_of_pre_morph' : proof.
 Require Import Setoid.
-
-Function appears (under_plus:bool) (v:nat) (f:formula) {struct f} : bool := 
-  match f with
-    | Proposition n => EqNat.beq_nat n v
-    | Otimes f1 f2  | And f1 f2 => 
-      orb (appears under_plus v f1) (appears under_plus v f2)
-    | Oplus f1 f2 | Implies f1 f2 => 
-      if under_plus 
-        then  orb (appears under_plus v f1) (appears under_plus v f2) 
-        else false
-    | Bang f => appears under_plus v f
-    | Zero => true
-    | _ => false
-  end.
-
-Definition exists_in_env f gamma := 
-  fold _ (fun k acc => orb (f k) acc) gamma false.
-
-Definition appears_in_env v := exists_in_env (appears true v).
-
-Lemma iter_bool_proper : forall v, Morphisms.Proper
-  (ILLVarInt.MILL.eq ==> Logic.eq ==> Logic.eq ==> Logic.eq)
-  (iter bool
-    (λ (k0 : formula) (acc : bool), (appears true v k0 || acc)%bool)).
+Add Morphism all_proofs_of with signature (eq ==> Logic.eq ==> iff) as
+all_proof_of_morph.
 Proof.
-  intros v.
-  red.
-  red.
-  intros x y H.
-  apply eq_is_eq in H.
-  subst.
-  red.
-  intros x y0 H.
-  subst.
-  red.
-  intros;subst;reflexivity.
+  intros x y H y0.
+  split;intros; eapply all_proofs_of_pre_morph;try eassumption.
+  apply eq_bool_complete;assumption.
+  apply eq_bool_complete;symmetry;assumption.
 Qed.
 
-  Lemma iter_transpose_nkey : forall v,MapsPtes.transpose_neqkey Logic.eq
-     (iter bool
-        (λ (k : formula) (acc : bool), (appears true v k || acc)%bool)).
-  Proof.
-  red.
-  intros v k k' e e' a _.
-  revert k' e' a.
-  induction e as [ | e].
-
-  simpl.
-  intros k' e'.
-  induction e' as [ | e'].
-  simpl;intros.
-  case(appears true v k);case (appears true v k');simpl;reflexivity. 
-  intros a.  
-  simpl.
-  rewrite <- IHe'.
-  case(appears true v k);case (appears true v k');simpl;reflexivity. 
-  intros k' e' a.
-  simpl.  
-  rewrite (IHe k' e').
-  f_equal.
-  case(appears true v k);simpl.
-  2:reflexivity.
-  clear.
-  induction e' as [|e'].
-  simpl.
-  auto with *.
-  simpl.
-  case (appears true v k');simpl;auto.
-Qed.
-
-Lemma appears_in_env_morph : ∀ v Γ Γ', Γ == Γ' -> appears_in_env v Γ = appears_in_env v Γ'.
-Proof.
-  intros v Γ Γ' H.
-  unfold appears_in_env, exists_in_env,fold.
-  revert Γ' H.
-  apply MapsPtes.fold_rec. 
-  Focus 1.
-  intros m H Γ' H0.
-  rewrite H0 in H.
-  rewrite MapsPtes.fold_Empty.
-  reflexivity.
-  auto.
-  assumption.
-  Unfocus.
-
-  Focus 1.
-  intros k e a m' m'' H H0 H1 H2 Γ' H3.
-  rewrite MapsPtes.fold_Add.
-  f_equal.
-  apply H2.
-  reflexivity.
-  auto.
-  apply iter_bool_proper.
-  apply iter_transpose_nkey.
-  assumption.
-  Focus 1. 
-  intro.
-  rewrite <- H3.
-  apply H1.
-  Unfocus.
-Qed.
-
-Add Morphism appears_in_env with signature (Logic.eq ==> eq ==> Logic.eq) as morph_appears_in_env.
-  exact appears_in_env_morph.
-Qed.
-
-Lemma appears_false_is_appears_true : forall n p, appears false n p = true -> appears true n p = true.
-Proof.
-  intros n p.
-  functional induction (appears false n p);simpl.
-  tauto.
-  intros H.  
-  rewrite Bool.orb_true_iff in H;destruct H.
-  rewrite IHb0;auto.
-  rewrite IHb1;auto with *.
-  intros H.  
-  rewrite Bool.orb_true_iff in H;destruct H.
-  rewrite IHb0;auto.
-  rewrite IHb1;auto with *.
-  intros H.  
-  rewrite Bool.orb_true_iff in H;destruct H.
-  rewrite IHb0;auto.
-  rewrite IHb1;auto with *.
-  discriminate.
-  intros H.  
-  rewrite Bool.orb_true_iff in H;destruct H.
-  rewrite IHb0;auto.
-  rewrite IHb1;auto with *.
-  discriminate.
-  auto.
-  reflexivity.
-  discriminate.
-Qed.
-
-Lemma exists_in_env_in : forall f φ Γ, φ∈Γ -> f φ = true -> exists_in_env f Γ = true.
-Proof.
-  intros f φ Γ H H0.
-  revert φ H0 H.
-  unfold exists_in_env.
-  apply fold_rec_weak.
-
-  intros m m' a H H0 φ H1 H2.
-  rewrite <- H in H2;eauto.
-
-  intros φ H0 H.  
-  unfold mem in H.
-  rewrite MapsPtes.F.empty_a in H;assumption.
-
-  intros k a m H φ H0 H1.
-  destruct (mem_destruct _ _ _ H1) as [H2|H2].
-  apply eq_is_eq in H2;subst.
-  rewrite H0;reflexivity.
-  rewrite H with (φ:=φ).
-  auto with *.
-  assumption.
-  assumption.
-Qed.
-
-Lemma in_exists_in_env : forall f Γ, exists_in_env f Γ = true -> exists φ,φ∈Γ/\ f φ = true.
-Proof.
-  intros f Γ.
-  unfold exists_in_env.
-  apply fold_rec_weak.
-
-  intros m m' a H H0 H1.
-  destruct (H0 H1) as [φ H2].
-  rewrite H in H2.
-  exists φ;assumption.
-
-  discriminate.
-
-  intros k a m H H0.
-  rewrite Bool.orb_true_iff in H0.
-  destruct H0.
-  exists k;split;auto.
-  apply add_is_mem;apply FormulaOrdered.eq_refl.
-  destruct (H H0) as [φ [H1 H2]].
-  exists φ;split.
-  apply mem_add_comm;assumption.
-  assumption.
-Qed.
-
-Lemma not_exists_in_env_in : forall f Γ, exists_in_env f Γ = false -> forall φ, φ∈Γ -> f φ = false.
-Proof.
-  intros f Γ.
-  unfold exists_in_env.
-  apply fold_rec_weak.
-
-  intros m m' a H H0 H1 φ H2.
-  rewrite <- H in H2;auto.
-
-  intros H φ H0.
-  unfold mem in H0;rewrite MapsPtes.F.empty_a in H0.
-  discriminate.
-
-  intros k a m H H0 φ H1.
-  rewrite Bool.orb_false_iff in H0;destruct H0.
-  destruct (mem_destruct _ _ _ H1).
-  apply eq_is_eq in H3;subst.
-  assumption.
-  auto.
-Qed.
-
-Lemma in_not_exists_in_env : forall f Γ, (forall φ, φ∈Γ -> f φ = false) -> exists_in_env f Γ = false.
-Proof.
-  intros f Γ.
-  unfold exists_in_env.
-  apply fold_rec_weak.
-
-  intros m m' a H H0 H1.
-  apply H0. 
-  intros φ H2.
-  rewrite H in H2;auto.
-
-  reflexivity.
-
-  intros k a m H H0.
-  rewrite H.
-  replace (f k) with false.
-  reflexivity.
-  symmetry.
-  apply H0.
-  apply add_is_mem.
-  apply FormulaOrdered.eq_refl.
-  intros φ H1.
-  apply H0.
-  apply mem_add_comm;assumption.
-Qed.
-
-
-
-
-Lemma exists_in_env_add : forall f φ Γ, exists_in_env f (φ::Γ) = ((f φ)|| (exists_in_env f Γ))%bool.
-Proof.
-  intros f φ Γ.
-  case_eq (exists_in_env f (φ::Γ));intros Heq.
-  destruct (in_exists_in_env _ _ Heq) as [ψ [H1 H2]].
-  destruct (mem_destruct _ _ _ H1).
-  apply eq_is_eq in H;subst.
-  rewrite H2;reflexivity.
-  rewrite (exists_in_env_in _ _ _ H H2). 
-  auto with *.
-  assert (Heq':=not_exists_in_env_in _ _ Heq).
-  rewrite  in_not_exists_in_env.
-  rewrite Heq'.
-  reflexivity.
-  apply add_is_mem;apply FormulaOrdered.eq_refl.
-  intros φ0 H.
-  apply Heq';apply mem_add_comm;assumption.
-Qed.
-  
-Lemma appears_in_env_in_appears : forall n φ Γ, φ∈Γ -> appears true n φ = true -> appears_in_env n Γ=true.
-Proof.
-  intros n φ Γ.
-
-  unfold appears_in_env.
-  intros H H0.
-  apply exists_in_env_in with φ;assumption.
-Qed.
-
-Lemma appears_in_env_false_add : 
-  forall n (Γ:t) φ, appears_in_env n (φ::Γ)  = false -> 
-    appears_in_env n Γ = false /\ appears true n φ = false.
-Proof.
-  intros n Γ.
-
-  induction Γ using multiset_ind.
-
-  intros φ H0.
-  rewrite <- H in H0.
-  assert (H':=IHΓ1 _ H0).
-  rewrite H in H';assumption.
-
-  intros φ H.
-  case_eq (appears true n φ);intros Heq1.
-  unfold appears_in_env,exists_in_env,fold,add in H.
-  rewrite MapsPtes.F.empty_o in H.
-  symmetry in H.
-  rewrite MapsPtes.fold_add in H.
-  simpl in H.
-  rewrite Heq1 in H;discriminate.
-  auto.
-  apply iter_proper.
-  clear;repeat red.
-  intros x y H x0 y0 H0.
-  repeat red in H0.
-  apply eq_is_eq in H;subst;reflexivity.
-  apply iter_transpose_nkey.
-  rewrite MapsPtes.F.empty_in_iff;tauto.
-  auto.
-
-  intros φ H.
-  assert (H':=  not_exists_in_env_in _ _ H).
-  rewrite H' by (apply add_is_mem;apply FormulaOrdered.eq_refl).
-  split;auto.
-  apply in_not_exists_in_env.
-  intros φ0 H0.
-  apply H'.
-  apply mem_add_comm;assumption.
-Qed.
-
-Lemma appears_false_remove : ∀ n (Γ:t) φ, appears_in_env n Γ = false -> 
-  appears_in_env n (Γ\φ) = false.
-Proof.
-  intros v Γ φ.
-  induction Γ using multiset_ind.
-
-  rewrite H in IHΓ1;assumption.
-
-  rewrite remove_empty;tauto.
-  intros H.
-  destruct (appears_in_env_false_add _ _ _ H) as [H1 H2];clear H.
-  apply in_not_exists_in_env.
-  intros φ0 H.
-  case (FormulaOrdered.eq_dec x φ);intro Heq.
-  rewrite remove_same_add in H by (symmetry;assumption).
-  apply not_exists_in_env_in with (Γ:=Γ);assumption.
-  rewrite remove_diff_add in H by (intro abs;elim Heq;rewrite abs;reflexivity).
-  generalize (mem_destruct _ _ _ H);intros [H3|H3].
-  apply eq_is_eq in H3;subst; assumption.
-  assert (H':=IHΓ H1).
-  apply not_exists_in_env_in with (Γ:=Γ\φ); assumption.
-Qed.
-
-Lemma appears_false_union : 
-  ∀ n Δ Δ', appears_in_env n (Δ∪Δ') = false -> 
-  appears_in_env n (Δ) = false /\ 
-  appears_in_env n (Δ') = false.
-Proof.
-  intros n Δ Δ' H.
-  split;apply in_not_exists_in_env;intros.
-  apply not_exists_in_env_in with (Γ:=Δ∪Δ');try assumption.
-  apply mem_union_l;assumption.
-  apply not_exists_in_env_in with (Γ:=Δ∪Δ');try assumption.
-  apply mem_union_r;assumption.
-Qed.
-
-Lemma var_in_env : ∀ Γ φ n, (appears false n φ) = true -> appears_in_env n Γ = false -> Γ⊢φ -> False.
-Proof.
-  intros Γ φ n H H0 H1.
-  revert H H0.
-
-  induction H1;intros  Heq1 Heq2;simpl in *;try discriminate.
-
-  Focus 1.
-  rewrite H in Heq2.
-  unfold appears_in_env,exists_in_env,fold,Maps'.fold in Heq2. simpl in Heq2.
-  apply appears_false_is_appears_true in Heq1.
-  rewrite Heq1 in Heq2.
-  discriminate Heq2.
-
-  Focus 1.
-  apply IHILL_proof2.
-  assumption.
-  assert (Heq2' := Heq2).
-  apply (appears_false_remove _ _ (p⊸q)) in Heq2.
-  rewrite H0 in Heq2.
-  apply appears_false_union in Heq2.
-  destruct Heq2.
-  apply in_not_exists_in_env.
-  intros φ H3.
-  destruct (mem_destruct _ _ _ H3) as [H4|H4].
-  apply eq_is_eq in H4;subst.
-  assert (appears true n (p⊸q) = false).
-  apply not_exists_in_env_in with (Γ:=Γ); assumption.
-  simpl in H4.
-  rewrite Bool.orb_false_iff in H4;intuition.
-  apply not_exists_in_env_in with (Γ:=Δ'); assumption.
-
-  Focus.
-  rewrite H in Heq2.
-  apply appears_false_union in Heq2;destruct Heq2.
-  rewrite Bool.orb_true_iff in Heq1;destruct Heq1.
-  apply IHILL_proof1;assumption.
-  apply IHILL_proof2;assumption.
-
-  Focus.
-  apply IHILL_proof.
-  assumption.
-  assert (Heq2' := Heq2).
-  apply (appears_false_remove _ _ (p⊗q)) in Heq2.
-  apply in_not_exists_in_env.
-  intros φ H3.
-  assert (appears true n (p⊗q) = false) by
-    (apply not_exists_in_env_in with (Γ:=Γ);assumption).
-  simpl in H0.
-  rewrite Bool.orb_false_iff in H0;intuition.
-  destruct (mem_destruct _ _ _ H3) as [H5|H5].
-  apply eq_is_eq in H5;subst;assumption.
-  destruct (mem_destruct _ _ _ H5) as [H6|H6].
-  apply eq_is_eq in H6;subst;assumption.
-  apply not_exists_in_env_in with (Γ:=Γ\p⊗q); assumption.
-
-  Focus.
-  apply IHILL_proof.
-  assumption.
-  assert (Heq2' := Heq2).
-  apply (appears_false_remove _ _ 1) in Heq2.
-  assumption.
-
-  Focus.
-  rewrite Bool.orb_true_iff in Heq1;destruct Heq1; eauto.
-
-  Focus.
-  apply IHILL_proof.
-  assumption.
-  assert (Heq2' := Heq2).
-  apply (appears_false_remove _ _ (p&q)) in Heq2.
-  apply in_not_exists_in_env.
-  intros φ H3.
-  assert (appears true n (p&q) = false) by
-    (apply not_exists_in_env_in with (Γ:=Γ);assumption).
-  simpl in H0.
-  rewrite Bool.orb_false_iff in H0;intuition.
-  destruct (mem_destruct _ _ _ H3) as [H5|H5].
-  apply eq_is_eq in H5;subst;assumption.
-  apply not_exists_in_env_in with (Γ:=Γ\p&q); assumption.
-
-  Focus.
-  apply IHILL_proof.
-  assumption.
-  assert (Heq2' := Heq2).
-  apply (appears_false_remove _ _ (p&q)) in Heq2.
-  apply in_not_exists_in_env.
-  intros φ H3.
-  assert (appears true n (p&q) = false) by
-    (apply not_exists_in_env_in with (Γ:=Γ);assumption).
-  simpl in H0.
-  rewrite Bool.orb_false_iff in H0;intuition.
-  destruct (mem_destruct _ _ _ H3) as [H5|H5].
-  apply eq_is_eq in H5;subst;assumption.
-  apply not_exists_in_env_in with (Γ:=Γ\p&q); assumption.
-
-  Focus.
-  apply IHILL_proof1.
-  assumption.
-  assert (Heq2' := Heq2).
-  apply (appears_false_remove _ _ (p⊕q)) in Heq2.
-  apply in_not_exists_in_env.
-  intros φ H3.
-  assert (appears true n (p⊕q) = false) by
-    (apply not_exists_in_env_in with (Γ:=Γ);assumption).
-  simpl in H0.
-  rewrite Bool.orb_false_iff in H0;intuition.
-  destruct (mem_destruct _ _ _ H3) as [H5|H5].
-  apply eq_is_eq in H5;subst;assumption.
-  apply not_exists_in_env_in with (Γ:=Γ\p⊕q); assumption.
-
-  Focus.
-  assert (H':=  not_exists_in_env_in _ _ Heq2).
-  generalize (H' _ H).
-  simpl;discriminate.
-
-  Focus.
-  apply IHILL_proof.
-  assumption.
-  assert (Heq2' := Heq2).
-  apply (appears_false_remove _ _ (!p)) in Heq2.
-  apply in_not_exists_in_env.
-  intros φ H3.
-  assert (appears true n (!p) = false) by
-    (apply not_exists_in_env_in with (Γ:=Γ);assumption).
-  simpl in H0.
-  destruct (mem_destruct _ _ _ H3) as [H5|H5].
-  apply eq_is_eq in H5;subst;assumption.
-  apply not_exists_in_env_in with (Γ:=Γ\!p); assumption.
-
-  Focus.
-  apply IHILL_proof.
-  assumption.
-  assert (Heq2' := Heq2).
-  apply (appears_false_remove _ _ (!p)) in Heq2.
-  apply in_not_exists_in_env.
-  intros φ H3.
-  assert (appears true n (!p) = false) by
-    (apply not_exists_in_env_in with (Γ:=Γ);assumption).
-  simpl in H0.
-  destruct (mem_destruct _ _ _ H3) as [H5|H5].
-  apply eq_is_eq in H5;subst;assumption.
-  apply not_exists_in_env_in with (Γ:=Γ); assumption.
-
-  Focus.
-  apply IHILL_proof.
-  assumption.
-  assert (Heq2' := Heq2).
-  apply (appears_false_remove _ _ (!p)) in Heq2.
-  apply in_not_exists_in_env.
-  intros φ H3.
-  assert (appears true n (!p) = false) by
-    (apply not_exists_in_env_in with (Γ:=Γ);assumption).
-  simpl in H0.
-  apply not_exists_in_env_in with (Γ:=Γ\!p); assumption.
-Qed.  
+Hint Extern 0 ( _ ==  _ ) => apply eq_bool_correct;vm_compute;reflexivity : proof.
 
 
 Ltac titi p := 
+  try complete eauto 2 with proof;
     (dependent simple inversion p||inversion p);clear p;subst;try discriminate;simpl.
 
-Ltac tutu :=
+
+Ltac decompose_add := 
+    repeat (match goal with 
+            | H : _ ∈ (_ :: _) |- _  => 
+              destruct (mem_destruct _ _ _ H);clear H
+            | H : _ ∈ ∅ |- _ => 
+              rewrite empty_no_mem in H;discriminate
+            | H : ILLVarInt.MILL.eq _ _ |- _ => apply eq_is_eq in H;subst
+          end).
+
+Ltac var_not_in_env_tac_simple n' H := 
+elim unusable_var_in_env with (n:=n') (1:=H);
+[
+  vm_compute;reflexivity |
+  vm_compute;reflexivity |
+  vm_compute;reflexivity |
+  vm_compute;reflexivity |
+    intros;decompose_add;simpl in *;repeat split;try discriminate;reflexivity
+]
+.
+
+Ltac var_not_in_env_tac_aux H env := 
+  match env with 
+    | Proposition ?n::?env' =>
+      (complete (var_not_in_env_tac_simple n H)) || 
+        var_not_in_env_tac_aux H env'
+    | _ :: ?env' =>  var_not_in_env_tac_aux H env'
+  end.
+
+Ltac var_not_in_env_tac H := 
+  match type of H with 
+    | ?env ⊢ _ => 
+      var_not_in_env_tac_aux H env
+  end.
+Ltac is_var_env gamma := 
+  match gamma with 
+    | empty => fail 1
+    | _ :: _ => fail 1
+    | _ \ _ => fail 1
+    | _ ∪ _ => fail 1
+    | _ => idtac
+  end.
+
+Ltac tutu := 
+  simpl;try reflexivity;
+    try discriminate;
+      try complete auto with proof;
+        (* try autorewrite with proof; *)
+          match goal with
+            | H : ?t == _ |- _ => 
+              is_var_env t;
+              match goal with 
+                | H': context [t] |- _ => 
+                  match H' with 
+                    | H => fail 1
+                    | _ => fail 2
+                  end
+                | _ => clear H
+              end
+          
+            | H : ?t = ?t |- _ => clear H
+            | H : ?t == ?t |- _ => clear H
+            | H:_ :: _ == _ ∪ _ |- _ => 
+              symmetry in H
+            | H: _ ∪ _ == _ :: _ |- _ => 
+              let delta := fresh "Δ" in
+                let h1 := fresh "H" in 
+                  let h2 := fresh "H" in 
+                    destruct (union_decompose _ _ _ _ H) 
+                      as [[delta [h1 h2]]|[delta [h1 h2]]];clear H
+            | H: empty == _ ∪ _ |- _ => 
+              symmetry in H
+            | H: _ ∪ _ == empty |- _ => 
+              let h1 := fresh "H" in 
+                let h2 := fresh "H" in 
+                  destruct (union_empty_decompose _ _  H) as [h1 h2];
+                    clear H
+         | H: ILLVarInt.MILL.eq _ _ |- _ => apply eq_is_eq in H; try (injection H;clear H;intros;subst)
+
+            | H: _ ∈ _ |- _ => complete (vm_compute in H;discriminate)
+            | H: _ ∈ (add _ _) |- _ =>   
+              destruct (mem_destruct _ _ _ H);clear H
+            | H : ?s == ?t |- _ => 
+              (complete (apply eq_bool_complete in H;vm_compute in H;
+                discriminate))|| (progress repeat (rewrite H in * ))
+            | H: context C [ remove ?f ?env ] |- _ => 
+              match env with 
+                context C' [ add f ?env' ] => 
+                let e := context C' [ env' ] in 
+                  setoid_replace (remove f env) with e in H by (apply eq_bool_correct;vm_compute;reflexivity)
+              end
+            | H:(?x ⊸ ?y) = _  |- _ => 
+              try discriminate H;injection H;clear H;intros;subst
+            | H: (_ ⊕ _) = _  |- _ => 
+              try discriminate H;injection H;clear H;intros;subst
+            | H:(_ ⊗ _) = _ |- _  => 
+              try discriminate H;injection H;clear H;intros;subst
+            | H: _  & _ = _  |- _  => 
+              try discriminate H;injection H;clear H;intros;subst
+            | H: _ = (?x ⊸ ?y) |- _ => 
+              try discriminate H;injection H;clear H;intros;subst
+            | H: _ = (_ ⊕ _) |- _ => 
+              try discriminate H;injection H;clear H;intros;subst
+            | H: _ = (_ ⊗ _) |- _  => 
+              try discriminate H;injection H;clear H;intros;subst
+            | H: _ = _  & _ |- _  => 
+              try discriminate H;injection H;clear H;intros;subst
+            | H: ?delta ⊢ _, H' : ?delta == ∅ |- _ => 
+              apply False_ind;rewrite H' in H;clear H';titi H;repeat tutu
+            | H: ?env⊢?g |- _ =>
+(*              try complete var_not_in_env_tac H; *)
+                match env with 
+                  | context C' [?env' \ ?f] => 
+                    match env' with 
+                      | context C [add f ?env''] => 
+                        let e' := context C [ env'' ] in 
+                          let e := context C' [ e' ] in 
+                            assert (heq: e == env) by (apply eq_bool_correct;vm_compute;reflexivity);
+                              symmetry in heq;
+                                let h := fresh "H" in 
+                                  let i' := fresh "i" in 
+                                    assert (h:(exists i':ILL_proof e g, Proof_eq.eq H i')) by (exists (ILL_proof_pre_morph _ _ _ heq H);
+                                      apply Proof_eq.sym;
+                                    apply Proof_eq.eq_pre_morph);
+          destruct h as [i' h];
+            rewrite exists_AtheseA_on_formula_proof_eq_compat with (h2:=i') (1:=h);
+              clear H h heq
+end
+end
+            | H: ?t == ?t', i: ?env⊢?f |- _ => 
+              match env with 
+                | context [ t ] => 
+                  let f_env := 
+                    match eval pattern t in env with
+                      | ?f _ => f
+                    end
+                    in
+                    let env'0 := constr:(f_env t')  in 
+                      let env' := eval cbv beta iota in env'0 in 
+                        let h := fresh "H" in 
+                          let i' := fresh "i" in 
+                            let heq := fresh "heq" in 
+                              assert (h:exists i': env'⊢f, Proof_eq.eq i i');[
+                                assert (heq:env'==env) by (rewrite H;reflexivity);
+                                  symmetry in heq;
+                                    exists (ILL_proof_pre_morph _ _ _ heq i);
+                                      apply Proof_eq.sym;apply Proof_eq.eq_pre_morph
+|
+  destruct h as [i' h];
+    rewrite exists_AtheseA_on_formula_proof_eq_compat with (h2:=i') (1:=h);clear i h;try (rewrite H in *;clear H)
+]
+end
+
+          end.
+
+
+Ltac finish := 
   simpl;try reflexivity;
     try discriminate;
     try complete auto with proof;
     try autorewrite with proof;
+      try complete (apply False_ind;auto with proof);
       match goal with 
-        | H: {_} == _ ∪ _ |- _ =>   
-          let h1 := fresh "H" in 
-            let h2 := fresh "H" in 
-              (symmetry in H;destruct (union_singleton_decompose _ _ _ H) as [[h1 h2]|[h1 h2]]);clear H
-        | H : ?t = ?t |- _ => clear H
-        | H: _ ∈ (add _ _) |- _ =>   destruct (mem_destruct _ _ _ H);clear H
-        | H: context C [ remove ?f ?env ] |- _ => 
-          match env with 
-            context C' [ add f ?env' ] => 
-            let e := context C' [ env' ] in 
-              setoid_replace (remove f env) with e in H by (apply eq_bool_correct;vm_compute;reflexivity)
-          end
-        | H : ?s == ?t |- _ => 
-          (complete (apply eq_bool_complete in H;vm_compute in H;discriminate))|| (progress repeat (rewrite H in *))
-        | H: _ ∈ _ |- _ => complete (vm_compute in H;discriminate)
-        | H: ILLVarInt.MILL.eq _ _ |- _ => apply eq_is_eq in H; try (injection H;clear H;intros;subst)
-        | H:(?x ⊸ ?y) = _  |- _ => try discriminate H;injection H;clear H;intros;subst
-        | H: (_ ⊕ _) = _  |- _ => try discriminate H;injection H;clear H;intros;subst
-        | H:(_ ⊗ _) = _ |- _  => try discriminate H;injection H;clear H;intros;subst
-        | H: _  & _ = _  |- _  => try discriminate H;injection H;clear H;intros;subst
-        | H: ?delta ⊢ _, H' : ?delta == ∅ |- _ => apply False_ind;rewrite H' in H;clear H';titi H;repeat tutu
-        | H: ?env⊢?g |- _ =>
-          match env with 
-            | context C' [?env' \ ?f] => 
-              match env' with 
-                | context C [add f ?env''] => 
-                  let e' := context C [ env'' ] in 
-                    let e := context C' [ e' ] in 
-                    assert (heq: e == env) by (apply eq_bool_correct;vm_compute;reflexivity);
-                      symmetry in heq;
-                        let h := fresh "H" in 
-                          let i' := fresh "i" in 
-                            assert (h:(exists i':ILL_proof e g, Proof_eq.eq H i')) by (exists (ILL_proof_pre_morph _ _ _ heq H);
-                              apply Proof_eq.sym;
-                            apply Proof_eq.eq_pre_morph);
-      destruct h as [i' h];
-        rewrite exists_AtheseA_on_formula_proof_eq_compat with (h2:=i') (1:=h);
-          clear H h heq
-end
-end
+        | |- (if ?e then trueP else trueP ) = trueP => 
+          case e;reflexivity
+        | H: ?env⊢?g |- _ => complete var_not_in_env_tac H
+        | i:?e⊢Proposition ?n' |- _ => 
+          elim var_in_env with (n:=n') (3:=i);vm_compute;reflexivity
+      end.
 
-    | H: ?t == ?t', i: ?env⊢?f |- _ => 
-      match env with 
-        | context [ t ] => 
-          let f_env := 
-            match eval pattern t in env with
-              | ?f _ => f
-            end
-            in
-          let env'0 := constr:(f_env t')  in 
-            let env' := eval cbv beta iota in env'0 in 
-            let h := fresh "H" in 
-              let i' := fresh "i" in 
-                let heq := fresh "heq" in 
-                  assert (h:exists i': env'⊢f, Proof_eq.eq i i');[
-                    assert (heq:env'==env) by (rewrite H;reflexivity);
-                      symmetry in heq;
-                        exists (ILL_proof_pre_morph _ _ _ heq i);
-                          apply Proof_eq.sym;apply Proof_eq.eq_pre_morph
-                    |
-                      destruct h as [i' h];
-                        rewrite exists_AtheseA_on_formula_proof_eq_compat with (h2:=i') (1:=h);clear i h;try (rewrite H in *;clear H)
-                      ]
-  end
-end.
-
-
-Ltac decompose_union := 
-  repeat 
-    match goal with 
-      | H:_ :: _ == _ ∪ _ |- _ => 
-        symmetry in H
-      | H: _ ∪ _ == _ :: _ |- _ => 
-        let delta := fresh "Δ" in
-          let h1 := fresh "H" in 
-            let h2 := fresh "H" in 
-              destruct (union_decompose _ _ _ _ H) as [[delta [h1 h2]]|[delta [h1 h2]]];clear H
-      | H: empty == _ ∪ _ |- _ => 
-        symmetry in H
-      | H: _ ∪ _ == empty |- _ => 
-        let h1 := fresh "H" in 
-          let h2 := fresh "H" in 
-            destruct (union_empty_decompose _ _  H) as [h1 h2];clear H
-    end.
-
-Ltac finish := 
-  match goal with 
-    |- (if ?e then trueP else trueP ) = trueP => 
-      case e;reflexivity
-    | i:?e⊢Proposition ?n' |- _ => 
-      elim var_in_env with (n:=n') (3:=i);vm_compute;reflexivity
-  end.
-
-Ltac swap e := 
-  match goal with 
-    | H : ?env⊢ ?g |-  _ =>
-      assert (heq: e == env) by (apply eq_bool_correct;vm_compute;reflexivity);
-        symmetry in heq;
-          let h := fresh "H" in 
-            let i' := fresh "i" in 
-              assert (h:(exists i':ILL_proof e g, Proof_eq.eq H i')) by (exists (ILL_proof_pre_morph _ _ _ heq H);
-                apply Proof_eq.sym;
-              apply Proof_eq.eq_pre_morph);
-destruct h as [i' h];
-  rewrite exists_AtheseA_on_formula_proof_eq_compat with (h2:=i') (1:=h);
-    clear H h heq; auto with proof
-end.
 
 Ltac one_step p :=   titi p; (repeat tutu);try finish.
 
+Ltac unusable_implies_tac n' f H := 
+  apply unusable_implies with (1:=H) (n:=n') (φ:=f);
+    [
+      vm_compute;reflexivity |
+        vm_compute;reflexivity |
+          vm_compute;reflexivity |
+            intros;decompose_add;repeat split;simpl in *;try discriminate;reflexivity].
 
-Notation "'all_proof_of' x" := (forall (p:x), exists_AtheseA_on_formula (fun _ _ _ => trueP) A M _ _ p =trueP) (at level 80,only parsing).
+Ltac unusable_var_strong_tac n1 n2 H :=
+  apply unusable_var_in_env_strong with (1:=H) (n:=n1);[
+  vm_compute;reflexivity|
+  vm_compute;reflexivity|
+  vm_compute;reflexivity|
+  vm_compute;reflexivity|
+  intros;decompose_add;simpl in *;  repeat split;try discriminate;try reflexivity;auto;
+  intros _;right;
+  exists n2;
+    split;[((left;reflexivity)||(right;reflexivity))|split;[
+      intros;decompose_add;simpl;reflexivity|vm_compute;reflexivity]]].
 
-Lemma proof_aux_1 : all_proof_of ({A} ⊢ A ⊕ M).
+
+(*
+Lemma aux_10 : no_proof_for ({E ⊸ A, P, (P ⊸ M) & 1, V}) V.
 Proof.
-  intros p;one_step p.
+  intro p;unusable_implies_tac 7%nat A p.
 Qed.
-Hint Resolve proof_aux_1 : proof.
-Hint Rewrite proof_aux_1 : proof.
+Hint Resolve aux_10 : proof.
 
-
-Lemma proof_1 : all_proof_of ({ (V⊸A),V}⊢A⊕M).
+Lemma aux_12 : no_proof_for ({P ⊸ M, P, V}) V.
 Proof.
-  intros p.
-  one_step p. 
+  intro p.
+  unusable_var_strong_tac 1%nat 8%nat p.
+Qed.
+Hint Resolve aux_12 : proof.
+
+Lemma aux_13 : no_proof_for ({1, P ⊸ M, P, V}) V.
+Proof.
+  intro p.
+  unusable_var_strong_tac 1%nat 8%nat p.
+Qed.
+Hint Resolve aux_13 : proof.
+
+Lemma aux_14 : no_proof_for ({P ⊸ M, P, (E ⊸ A) & 1, V}) V.
+Proof.
+  intro p.
+  unusable_var_strong_tac 1%nat 8%nat p.
+Qed.
+Hint Resolve aux_14 : proof.
+
+Lemma aux_16 : no_proof_for ({1, P, (P ⊸ M) & 1, V}) V.
+Proof.
+  intros p; one_step p;eauto with proof.
+Qed.
+Hint Resolve aux_16 : proof.
+
+Lemma aux_18 : no_proof_for ({E ⊸ A, A, P, (P ⊸ M) & 1}) (A ⊕ M).
+Proof.
+  intro p;unusable_implies_tac 7%nat A p.
+Qed.
+Hint Resolve aux_18 : proof.
+
+Lemma aux_19 : no_proof_for ({M, A}) (A ⊕ M).
+Proof.
+  intros p; one_step p;eauto with proof.
+Qed.
+Hint Resolve aux_19 : proof.
+
+Lemma aux_20 : no_proof_for ({E ⊸ A, M, A}) (A ⊕ M).
+Proof.
+  intro p;unusable_implies_tac 7%nat A p.
+Qed.
+Hint Resolve aux_20 : proof.
+
+Lemma aux_21 : no_proof_for ({1, M, A})(A ⊕ M).
+Proof.
+  intros p; one_step p;eauto with proof.
+Qed.
+Hint Resolve aux_21 : proof.
+
+Lemma aux_22 : no_proof_for ({M, A, (E ⊸ A) & 1}) (A ⊕ M).
+Proof.
+  intros p; one_step p;eauto with proof.
+Qed.
+Hint Resolve aux_22 : proof.
+
+Lemma aux_23 : no_proof_for ({E ⊸ A, P ⊸ M, A, P}) (A ⊕ M).
+Proof.
+  intro p;unusable_implies_tac 7%nat A p.
+Qed.
+Hint Resolve aux_23 : proof.
+
+Lemma aux_24 : no_proof_for ({P ⊸ M, A, P}) A.
+Proof.
+  intro p.
+  unusable_var_strong_tac 1%nat 8%nat p.
+Qed.
+Hint Resolve aux_24 : proof.
+
+Lemma aux_25 : no_proof_for ({P ⊸ M, A, P}) (A ⊕ M).
+Proof.
+  intros p; one_step p;eauto with proof.
+Qed.
+Hint Resolve aux_25 : proof.
+
+Lemma aux_26 : no_proof_for ({1, P ⊸ M, A, P}) A.
+Proof.
+  intro p.
+  unusable_var_strong_tac 1%nat 8%nat p.
+Qed.
+Hint Resolve aux_26 : proof.
+
+Lemma aux_27 : no_proof_for ({1, P ⊸ M, A, P}) (A ⊕ M).
+Proof.
+  intros p; one_step p;eauto with proof.
+(* 
+   {P ⊸ M, A, P} ⊢ A ⊕ M
+   {1, P ⊸ M, A, P} ⊢ A 
+*)
+Qed.
+Hint Resolve aux_27 : proof.
+
+Lemma aux_29 : no_proof_for ({P ⊸ M, A, P, (E ⊸ A) & 1}) A.
+Proof.
+  intro p.
+  unusable_var_strong_tac 1%nat 8%nat p.
+Qed.
+Hint Resolve aux_29 : proof.
+
+Lemma aux_30 : no_proof_for ({P ⊸ M, A, P, (E ⊸ A) & 1}) (A ⊕ M).
+Proof.
+  intros p; one_step p;eauto with proof.
+(*
+{M, A} ⊢ A ⊕ M
+{M, A, (E ⊸ A) & 1} ⊢ A ⊕ M
+{E ⊸ A, P ⊸ M, A, P} ⊢ A ⊕ M
+{1, P ⊸ M, A, P} ⊢ A ⊕ M
+{P ⊸ M, A, P, (E ⊸ A) & 1} ⊢ A e
+*)
+Qed.
+Hint Resolve aux_30 : proof.
+
+
+Lemma aux_31 : no_proof_for ({A, P, (P ⊸ M) & 1}) A.
+Proof.
+  intros p; one_step p;eauto with proof.
+Qed.
+Hint Resolve aux_31 : proof.
+
+Lemma aux_32 : no_proof_for ({A, P, (P ⊸ M) & 1}) (A ⊕ M).
+Proof.
+  intros p; one_step p;eauto with proof.
+(* ({A, P, (P ⊸ M) & 1}) A *)
+Qed.
+Hint Resolve aux_32 : proof.
+
+Lemma aux_33 : no_proof_for ({1, A, P, (P ⊸ M) & 1}) A.
+Proof.
+  intros p; one_step p;eauto with proof.
+Qed.
+Hint Resolve aux_33 : proof.
+
+Lemma aux_34 : no_proof_for ({1, A, P, (P ⊸ M) & 1}) (A ⊕ M).
+Proof.
+  intros p; one_step p;eauto with proof.
+(*
+ {A, P, (P ⊸ M) & 1} ⊢ A ⊕ M
+ {1, A, P, (P ⊸ M) & 1} ⊢ A
+*)
+Qed.
+Hint Resolve aux_34 : proof.
+
+
+Lemma aux_35 : no_proof_for ({E ⊸ A, A, P, (P ⊸ M) & 1}) A.
+Proof.
+  intro p;unusable_implies_tac 7%nat A p.
+Qed.
+Hint Resolve aux_35 : proof.
+ 
+Lemma aux_36 : no_proof_for ({A, P, (E ⊸ A) & 1, (P ⊸ M) & 1}) A.
+Proof.
+  intros p; one_step p;eauto with proof.
+(* 
+{E ⊸ A, A, P, (P ⊸ M) & 1} ⊢ A
+*)
+Qed.
+Hint Resolve aux_36 : proof.
+
+Lemma aux_38 : no_proof_for ({E ⊸ A, V ⊸ A, P, (P ⊸ M) & 1, V}) (A ⊕ M).
+Proof.
+  intro p;unusable_implies_tac 7%nat A p.
+Qed.
+Hint Resolve aux_38 : proof.
+
+Lemma aux_40 : no_proof_for ({V ⊸ A, P, V}) P.
+Proof.
+  intro p.
+  unusable_var_strong_tac 5%nat 6%nat p.
+Qed.
+Hint Resolve aux_40 : proof.
+
+Lemma aux_42 : no_proof_for ({V ⊸ A, P, (E ⊸ A) & 1, V}) P.
+Proof.
+  intro p.
+  unusable_var_strong_tac 5%nat 6%nat p.
+Qed.
+Hint Resolve aux_42 : proof.
+
+Lemma aux_43 : no_proof_for ({M, V ⊸ A, V}) M.
+Proof.
+  intro p.
+  unusable_var_strong_tac 5%nat 6%nat p.
+
+Qed.
+Hint Resolve aux_43 : proof.
+
+Lemma aux_44 : no_proof_for ({M, V ⊸ A, V}) (A ⊕ M).
+Proof.
+  intros p; one_step p;eauto with proof.
+(* 
+   {M, V ⊸ A, V} ⊢ M
+*)
+Qed.
+Hint Resolve aux_44 : proof.
+
+Lemma aux_45 : no_proof_for ({E ⊸ A, M, V ⊸ A, V}) (A ⊕ M).
+Proof.
+  intro p;unusable_implies_tac 7%nat A p.
+Qed.
+Hint Resolve aux_45 : proof.
+
+Lemma aux_46 : no_proof_for ({1, M, V ⊸ A, V}) (M).
+Proof.
+  intro p.
+  unusable_var_strong_tac 5%nat 6%nat p.
+Qed.
+Hint Resolve aux_46 : proof.
+
+Lemma aux_47 : no_proof_for ({1, M, V ⊸ A, V}) (A ⊕ M).
+Proof.
+  intros p; one_step p;eauto with proof.
+Qed.
+Hint Resolve aux_47 : proof.
+
+Lemma aux_49 : no_proof_for ({M, V ⊸ A, (E ⊸ A) & 1, V}) M.
+Proof.
+  intro p.
+  unusable_var_strong_tac 5%nat 6%nat p.
+Qed.
+Hint Resolve aux_49 : proof.
+
+Lemma aux_50 : no_proof_for ({M, V ⊸ A, (E ⊸ A) & 1, V}) (A ⊕ M).
+Proof.
+  intros p; one_step p;eauto with proof.
+(*
+ {E ⊸ A, M, V ⊸ A, V} ⊢ A ⊕ M
+ {1, M, V ⊸ A, V} ⊢ A ⊕ M
+ {M, V ⊸ A, (E ⊸ A) & 1, V} ⊢ M 
+*)
+Qed.
+Hint Resolve aux_50 : proof.
+
+Lemma aux_41 : no_proof_for ({1, V ⊸ A, P, V}) P.
+Proof.
+  intro p.
+  unusable_var_strong_tac 5%nat 6%nat p.
+Qed.
+Hint Resolve aux_41 : proof.
+
+Lemma aux_52 : no_proof_for ({P ⊸ M, V ⊸ A, P, V}) A.
+Proof.
+  intro p.
+  unusable_var_strong_tac 1%nat 8%nat p.
+Qed.
+Hint Resolve aux_52 : proof.
+
+Lemma aux_53 : no_proof_for ({P ⊸ M, V ⊸ A, P, V}) M.
+Proof.
+  intro p.
+  unusable_var_strong_tac 5%nat 6%nat p.
+Qed.
+Hint Resolve aux_53 : proof.
+
+Lemma aux_54 : no_proof_for ({P ⊸ M, V ⊸ A, P, V}) (A ⊕ M).
+Proof.
+  intros p; one_step p;eauto with proof.
+(*
+   {P ⊸ M, V ⊸ A, P, V} ⊢ A
+   {P ⊸ M, V ⊸ A, P, V} ⊢ M
+*)
+Qed.
+Hint Resolve aux_54 : proof.
+
+
+Lemma aux_55 : no_proof_for ({1, P ⊸ M, V ⊸ A, P, V}) A.
+Proof.
+  intro p.
+  unusable_var_strong_tac 1%nat 8%nat p.
+Qed.
+Hint Resolve aux_55 : proof.
+
+Lemma aux_56 : no_proof_for ({1, P ⊸ M, V ⊸ A, P, V}) M.
+Proof.
+  intro p.
+  unusable_var_strong_tac 5%nat 6%nat p.
+Qed.
+Hint Resolve aux_56 : proof.
+
+Lemma aux_57 : no_proof_for  ({1, P ⊸ M, V ⊸ A, P, V}) (A ⊕ M).
+Proof.
+  intros p; one_step p;eauto with proof.
+(*
+{1, V ⊸ A, P, V} ⊢ P 
+{P ⊸ M, V ⊸ A, P, V} ⊢ A ⊕ M
+{1, P ⊸ M, V ⊸ A, P, V} ⊢ A 
+{1, P ⊸ M, V ⊸ A, P, V} ⊢ M
+*)
+Qed.
+Hint Resolve aux_57 : proof.
+
+Lemma aux_59 : no_proof_for ({P ⊸ M, V ⊸ A, P, (E ⊸ A) & 1, V}) A.
+Proof.
+  intro p.
+  unusable_var_strong_tac 1%nat 8%nat p.
+Qed.
+Hint Resolve aux_59 : proof.
+
+Lemma aux_60 : no_proof_for ({E ⊸ A, P ⊸ M, V ⊸ A, P, V}) M.
+Proof.
+  intro p;unusable_implies_tac 7%nat A p.
+Qed.
+Hint Resolve aux_60 : proof.
+
+Lemma aux_61 : no_proof_for ({P ⊸ M, V ⊸ A, P, (E ⊸ A) & 1, V}) M.
+Proof.
+  intro p.
+  unusable_var_strong_tac 5%nat 6%nat p.
+Qed.
+Hint Resolve aux_61 : proof.
+
+Lemma aux_51 : no_proof_for ({E ⊸ A, P ⊸ M, V ⊸ A, P, V}) (A ⊕ M).
+Proof.
+  intro p;unusable_implies_tac 7%nat A p.
+Qed.
+Hint Resolve aux_51 : proof.
+
+Lemma aux_62 : no_proof_for ({P ⊸ M, V ⊸ A, P, (E ⊸ A) & 1, V}) (A ⊕ M).
+Proof.
+  intros p; one_step p;eauto with proof.
+(*
+ {V ⊸ A, P, (E ⊸ A) & 1, V} ⊢ P e
+ {V ⊸ A, P, V} ⊢ P e
+ {M, V ⊸ A, V} ⊢ A ⊕ M
+ {M, V ⊸ A, (E ⊸ A) & 1, V} ⊢ A ⊕ M
+ {E ⊸ A, P ⊸ M, V ⊸ A, P, V} ⊢ A ⊕ M
+ {1, P ⊸ M, V ⊸ A, P, V} ⊢ A ⊕ M
+ {P ⊸ M, V ⊸ A, P, (E ⊸ A) & 1, V} ⊢ A e
+ {P ⊸ M, V ⊸ A, P, (E ⊸ A) & 1, V} ⊢ M e
+ *)
+Qed.
+Hint Resolve aux_62 : proof.
+
+
+Lemma aux_63 : no_proof_for ({V ⊸ A, P, (P ⊸ M) & 1, V}) A.
+Proof.
+  intros p; one_step p;eauto with proof.
+Qed.
+Hint Resolve aux_63 : proof.
+
+Lemma aux_64 : no_proof_for ({V ⊸ A, P, (P ⊸ M) & 1, V}) M.
+Proof.
+  intro p.
+  unusable_var_strong_tac 5%nat 6%nat p.
+Qed.
+Hint Resolve aux_64 : proof.
+
+Lemma aux_65 : no_proof_for ({V ⊸ A, P, (P ⊸ M) & 1, V}) (A ⊕ M).
+Proof.
+  intros p; one_step p;eauto with proof.
+(*
+ {V ⊸ A, P, (P ⊸ M) & 1, V} ⊢ A
+ {V ⊸ A, P, (P ⊸ M) & 1, V} ⊢ M e
+*)
+Qed.
+Hint Resolve aux_65 : proof.
+
+Lemma aux_66 : no_proof_for ({1, V ⊸ A, P, (P ⊸ M) & 1, V}) A.
+Proof.
+  intros p; one_step p;eauto with proof.
+Qed.
+Hint Resolve aux_66 : proof.
+
+Lemma aux_67 : no_proof_for ({1, V ⊸ A, P, (P ⊸ M) & 1, V}) M.
+Proof.
+  intro p.
+  unusable_var_strong_tac 5%nat 6%nat p.
+Qed.
+Hint Resolve aux_67 : proof.
+
+Lemma aux_68 : no_proof_for ({1, V ⊸ A, P, (P ⊸ M) & 1, V}) (A ⊕ M).
+Proof.
+  intros p; one_step p;eauto with proof.
+(*
+ {V ⊸ A, P, (P ⊸ M) & 1, V} ⊢ A ⊕ M
+ {1, V ⊸ A, P, (P ⊸ M) & 1, V} ⊢ A
+ {1, V ⊸ A, P, (P ⊸ M) & 1, V} ⊢ M e
+*)
+Qed.
+Hint Resolve aux_68 : proof.
+
+Lemma aux_69 : no_proof_for ({E ⊸ A, V ⊸ A, P, (P ⊸ M) & 1, V}) A.
+Proof.
+  intro p;unusable_implies_tac 7%nat A p.
+Qed.
+Hint Resolve aux_69 : proof.
+
+Lemma aux_70 : no_proof_for ({V ⊸ A, P, (E ⊸ A) & 1, (P ⊸ M) & 1, V}) A.
+Proof.
+  intros p; one_step p;eauto with proof.
+(*
+   {E ⊸ A, V ⊸ A, P, (P ⊸ M) & 1, V} ⊢ A     
+*)
+Qed.
+Hint Resolve aux_70 : proof.
+
+Lemma aux_72 : no_proof_for ({V ⊸ A, P, (E ⊸ A) & 1, (P ⊸ M) & 1, V}) M.
+Proof.
+  intro p.
+  unusable_var_strong_tac 5%nat 6%nat p.
+Qed.
+Hint Resolve aux_72 : proof.
+
+Lemma aux_74 : no_proof_for ({E ⊸ A, P, (V ⊸ A) & 1, (P ⊸ M) & 1, V}) (A ⊕ M).
+Proof.
+  intro p;unusable_implies_tac 7%nat A p.
+Qed.
+Hint Resolve aux_74 : proof.
+
+Lemma aux_75 : no_proof_for ({E ⊸ A, P, (V ⊸ A) & 1, V}) P.
+Proof.
+  intro p;unusable_implies_tac 7%nat A p.
+Qed.
+Hint Resolve aux_75 : proof.
+
+Lemma aux_76 : no_proof_for ({P, (V ⊸ A) & 1, V}) P.
+Proof.
+  intros p; one_step p;eauto with proof.
+Qed.
+Hint Resolve aux_76 : proof.
+
+Lemma aux_77 : no_proof_for ({1, P, (V ⊸ A) & 1, V}) P.
+Proof.
+  intros p; one_step p;eauto with proof.
+(*
+ {P, (V ⊸ A) & 1, V} ⊢ P
+*)
+Qed.
+Hint Resolve aux_77 : proof.
+
+Lemma aux_78 : no_proof_for ({P, (V ⊸ A) & 1, (E ⊸ A) & 1, V}) P.
+Proof.
+  intros p; one_step p;eauto with proof.
+(*
+ {E ⊸ A, P, (V ⊸ A) & 1, V} ⊢ P
+ {1, P, (V ⊸ A) & 1, V} ⊢ P
+*)
+Qed.
+Hint Resolve aux_78 : proof.
+
+Lemma aux_79 : no_proof_for ({E ⊸ A, M, (V ⊸ A) & 1, V}) (A ⊕ M).
+Proof.
+  intro p;unusable_implies_tac 7%nat A p.
+Qed.
+Hint Resolve aux_79 : proof.
+
+Lemma aux_80 : no_proof_for ({M, (V ⊸ A) & 1, V}) (M).
+Proof.
+  intros p; one_step p;eauto with proof.
+Qed.
+Hint Resolve aux_80 : proof.
+
+Lemma aux_88 : no_proof_for ({M, (V ⊸ A) & 1, V}) (A ⊕ M).
+Proof.
+  intros p; one_step p;eauto with proof.
+(*
+   {M, (V ⊸ A) & 1, V} ⊢ M
+*)
+Qed.
+Hint Resolve aux_88 : proof.
+
+Lemma aux_82 : no_proof_for ({1, M, (V ⊸ A) & 1, V}) M.
+Proof.
+  intros p; one_step p;eauto with proof.
+Qed.
+Hint Resolve aux_82 : proof.
+
+Lemma aux_83 : no_proof_for ({1, M, (V ⊸ A) & 1, V}) (A ⊕ M).
+Proof.
+  intros p; one_step p;eauto with proof.
+(*
+ {M, (V ⊸ A) & 1, V} ⊢ A ⊕ M
+ {1, M, (V ⊸ A) & 1, V} ⊢ M
+*)
+Qed.
+Hint Resolve aux_83 : proof.
+
+Lemma aux_87 : no_proof_for ({E ⊸ A, M, (V ⊸ A) & 1, V}) M.
+Proof.
+  intro p;unusable_implies_tac 7%nat A p.
+Qed.
+Hint Resolve aux_87 : proof.
+
+Lemma aux_85 : no_proof_for ({M, (V ⊸ A) & 1, (E ⊸ A) & 1, V}) M.
+Proof.
+  intros p; one_step p;eauto with proof.
+(*
+{E ⊸ A, M, (V ⊸ A) & 1, V} ⊢ M
+*)
+Qed.
+Hint Resolve aux_85 : proof.
+
+Lemma aux_86 : no_proof_for ({M, (V ⊸ A) & 1, (E ⊸ A) & 1, V}) (A ⊕ M).
+Proof.
+  intros p; one_step p;eauto with proof.
+(*
+{E ⊸ A, M, (V ⊸ A) & 1, V} ⊢ A ⊕M 
+{1, M, (V ⊸ A) & 1, V} ⊢ A ⊕ M
+{M, (V ⊸ A) & 1, (E ⊸ A) & 1, V} ⊢ M
+*)
+Qed.
+Hint Resolve aux_86 : proof.
+
+Lemma aux_89 : no_proof_for ({E ⊸ A, P ⊸ M, P, (V ⊸ A) & 1, V}) (A ⊕ M).
+Proof.
+  intro p;unusable_implies_tac 7%nat A p.
+Qed.
+Hint Resolve aux_89 : proof.
+
+Lemma aux_90 : no_proof_for ({P ⊸ M, P, (V ⊸ A) & 1, V}) A.
+Proof.
+  intro p.
+  unusable_var_strong_tac 1%nat 8%nat p.
+Qed.
+Hint Resolve aux_90 : proof.
+
+Lemma aux_91 : no_proof_for ({P ⊸ M, P, (V ⊸ A) & 1, V}) M.
+Proof.
+  intros p; one_step p;eauto with proof.
+Qed.
+Hint Resolve aux_91 : proof.
+
+Lemma aux_92 : no_proof_for ({P ⊸ M, P, (V ⊸ A) & 1, V}) (A ⊕ M).
+Proof.
+  intros p; one_step p;eauto with proof.
+(*
+{P ⊸ M, P, (V ⊸ A) & 1, V} ⊢ A e
+{P ⊸ M, P, (V ⊸ A) & 1, V} ⊢ M
+*)
+Qed.
+Hint Resolve aux_92 : proof.
+
+Lemma aux_93 : no_proof_for ({1, P ⊸ M, P, (V ⊸ A) & 1, V}) A.
+Proof.
+  intro p.
+  unusable_var_strong_tac 1%nat 8%nat p.
+Qed.
+Hint Resolve aux_93 : proof.
+
+Lemma aux_94 : no_proof_for ({1, P ⊸ M, P, (V ⊸ A) & 1, V}) M.
+Proof.
+  intros p; one_step p;eauto with proof.
+Qed.
+Hint Resolve aux_94 : proof.
+
+Lemma aux_95 : no_proof_for ({1, P ⊸ M, P, (V ⊸ A) & 1, V}) (A ⊕ M).
+Proof.
+  intros p; one_step p;eauto with proof.
+(*
+{P ⊸ M, P, (V ⊸ A) & 1, V} ⊢ A ⊕ M
+{1, P ⊸ M, P, (V ⊸ A) & 1, V} ⊢ A e
+{1, P ⊸ M, P, (V ⊸ A) & 1, V} ⊢ M
+*)
+Qed.
+Hint Resolve aux_95 : proof.
+
+Lemma aux_97 : no_proof_for ({P ⊸ M, P, (V ⊸ A) & 1, (E ⊸ A) & 1, V}) A.
+Proof.
+  intro p.
+  unusable_var_strong_tac 1%nat 8%nat p.
+Qed.
+Hint Resolve aux_97 : proof.
+
+Lemma aux_98 : no_proof_for ({E ⊸ A, P ⊸ M, P, (V ⊸ A) & 1, V}) M.
+Proof.
+  intro p;unusable_implies_tac 7%nat A p.
+Qed.
+Hint Resolve aux_98 : proof.
+
+Lemma aux_99 : no_proof_for ({P ⊸ M, P, (V ⊸ A) & 1, (E ⊸ A) & 1, V}) M.
+Proof.
+  intros p; one_step p;eauto with proof.
+(*
+{E ⊸ A, P ⊸ M, P, (V ⊸ A) & 1, V} ⊢ M
+*)
+Qed.
+Hint Resolve aux_99 : proof.
+
+Lemma aux_100 : no_proof_for ({P ⊸ M, P, (V ⊸ A) & 1, (E ⊸ A) & 1, V}) (A ⊕ M).
+Proof.
+  intros p; one_step p;eauto with proof.
+(*
+{P, (V ⊸ A) & 1, (E ⊸ A) & 1, V} ⊢ P
+{P, (V ⊸ A) & 1, V} ⊢ P
+{M, (V ⊸ A) & 1, (E ⊸ A) & 1, V} ⊢ A ⊕ M
+{M, (V ⊸ A) & 1, V} ⊢ A ⊕ M
+{E ⊸ A, P ⊸ M, P, (V ⊸ A) & 1, V} ⊢ A ⊕ M
+{1, P ⊸ M, P, (V ⊸ A) & 1, V} ⊢ A ⊕ M
+{P ⊸ M, P, (V ⊸ A) & 1, (E ⊸ A) & 1, V} ⊢ A e
+ {P ⊸ M, P, (V ⊸ A) & 1, (E ⊸ A) & 1, V} ⊢ M
+*)
+Qed.
+Hint Resolve aux_100 : proof.
+
+Lemma aux_101 : no_proof_for ({P, (V ⊸ A) & 1, (P ⊸ M) & 1, V}) A.
+Proof.
+  intros p; one_step p;eauto with proof.
+Qed.
+Hint Resolve aux_101 : proof.
+
+Lemma aux_102 : no_proof_for ({P, (V ⊸ A) & 1, (P ⊸ M) & 1, V}) M.
+Proof.
+  intros p; one_step p;eauto with proof.
+Qed.
+Hint Resolve aux_102 : proof.
+
+Lemma aux_103 : no_proof_for ({P, (V ⊸ A) & 1, (P ⊸ M) & 1, V}) (A ⊕ M).
+Proof.
+  intros p; one_step p;eauto with proof.
+(*
+{P, (V ⊸ A) & 1, (P ⊸ M) & 1, V} ⊢ A
+{P, (V ⊸ A) & 1, (P ⊸ M) & 1, V} ⊢ M
+*)
+Qed.
+Hint Resolve aux_103 : proof.
+
+Lemma aux_104 : no_proof_for ({1, P, (V ⊸ A) & 1, (P ⊸ M) & 1, V}) A.
+Proof.
+  intros p; one_step p;eauto with proof.
+Qed.
+Hint Resolve aux_104 : proof.
+
+Lemma aux_105 : no_proof_for ({1, P, (V ⊸ A) & 1, (P ⊸ M) & 1, V}) M.
+Proof.
+  intros p; one_step p;eauto with proof.
+Qed.
+Hint Resolve aux_105 : proof.
+
+Lemma aux_106 : no_proof_for ({1, P, (V ⊸ A) & 1, (P ⊸ M) & 1, V}) (A ⊕ M).
+Proof.
+  intros p; one_step p;eauto with proof.
+(*
+{P, (V ⊸ A) & 1, (P ⊸ M) & 1, V} ⊢ A ⊕ M
+{1, P, (V ⊸ A) & 1, (P ⊸ M) & 1, V} ⊢ A
+{1, P, (V ⊸ A) & 1, (P ⊸ M) & 1, V} ⊢ M
+*)
+Qed.
+Hint Resolve aux_106 : proof.
+
+Lemma aux_107 : no_proof_for ({E ⊸ A, P, (V ⊸ A) & 1, (P ⊸ M) & 1, V}) A.
+Proof.
+  intro p;unusable_implies_tac 7%nat A p.
+Qed.
+Hint Resolve aux_107 : proof.
+
+Lemma aux_108 : no_proof_for ({P, (V ⊸ A) & 1, (E ⊸ A) & 1, (P ⊸ M) & 1, V}) A.
+Proof.
+  intros p; one_step p;eauto with proof.
+(*
+{E ⊸ A, P, (V ⊸ A) & 1, (P ⊸ M) & 1, V} ⊢ A
+*)
+Qed.
+Hint Resolve aux_108 : proof.
+
+Lemma aux_109 : no_proof_for ({E ⊸ A, P, (V ⊸ A) & 1, (P ⊸ M) & 1, V}) M.
+Proof.
+  intro p;unusable_implies_tac 7%nat A p.
+Qed.
+Hint Resolve aux_109 : proof.
+
+Lemma aux_110 : no_proof_for ({P, (V ⊸ A) & 1, (E ⊸ A) & 1, (P ⊸ M) & 1, V}) M.
+Proof.
+  intros p; one_step p;eauto with proof.
+Qed.
+Hint Resolve aux_110 : proof.
+
+Lemma aux_200 : no_proof_for ({P ⊸ M, A}) (A ⊕ M).
+Proof.
+  intro p;unusable_implies_tac 1%nat M p.
+Qed.
+Hint Resolve aux_200 : proof.
+
+Lemma aux_201 : all_proofs_of ({A, (P ⊸ M) & 1}) (A ⊕ M).
+Proof.
+  intros p; one_step p;eauto with proof.
+(*
+{P ⊸ M, A} ⊢ A ⊕ M -
+*)
+Qed.
+Hint Resolve aux_201 : proof.
+
+Lemma aux_202 : no_proof_for ({E ⊸ A, A, (P ⊸ M) & 1}) (A ⊕ M). 
+Proof.
+  intro p;unusable_implies_tac 7%nat A p.
+Qed.
+Hint Resolve aux_202 : proof.
+
+Lemma aux_203 : no_proof_for ({P ⊸ M, A, (E ⊸ A) & 1}) (A ⊕ M).
+Proof.
+  intro p;unusable_implies_tac 1%nat M p.
+Qed.
+Hint Resolve aux_203 : proof.
+
+Lemma aux_204 : no_proof_for ({P ⊸ M, 1, A}) (A ⊕ M).
+Proof.
+  intro p;unusable_implies_tac 1%nat M p.
+Qed.
+Hint Resolve aux_204 : proof.
+
+Lemma aux_205 : all_proofs_of ({1, A, (P ⊸ M) & 1}) (A ⊕ M).
+Proof.
+  intros p; one_step p;eauto with proof.
+(* 
+{P ⊸ M, 1, A} ⊢ A ⊕ M
+ *)
+Qed.
+Hint Resolve aux_205 : proof.
+Hint Rewrite aux_205 : proof.
+
+Lemma aux_206 : no_proof_for ({E ⊸ A, A}) (A ⊕ M).
+Proof.
+  intro p;unusable_implies_tac 7%nat A p.
+Qed.
+Hint Resolve aux_206 : proof.
+
+Lemma aux_207 : all_proofs_of ({A, (E ⊸ A) & 1}) (A ⊕ M).
+Proof.
+  intros p; one_step p;eauto with proof.
+(* 
+   {E ⊸ A, A} ⊢ A ⊕ M
+*)
+Qed.
+Hint Resolve aux_207 : proof.
+Hint Rewrite aux_207 : proof.
+
+Lemma aux_208 : no_proof_for ({E ⊸ A, 1, A}) (A ⊕ M).
+Proof.
+  intro p;unusable_implies_tac 7%nat A p.
+Qed.
+Hint Resolve aux_208 : proof.
+
+Lemma aux_209 : all_proofs_of ({1, A, (E ⊸ A) & 1}) (A ⊕ M).
+Proof.
+  intros p; one_step p;eauto with proof.
+(* 
+   {A, (E ⊸ A) & 1} ⊢ A ⊕ M + 
+   {E ⊸ A, 1, A} ⊢ A ⊕ M - e
+
+*)
+Qed.
+Hint Resolve aux_209 : proof.
+Hint Rewrite aux_209 : proof.
+
+Lemma aux_210 : all_proofs_of ({A, (E ⊸ A) & 1, (P ⊸ M) & 1}) (A ⊕ M).
+Proof.
+  intros p; one_step p;eauto with proof.
+(*
+{E ⊸ A, A, (P ⊸ M) & 1} ⊢ A ⊕ M - e
+{P ⊸ M, A, (E ⊸ A) & 1} ⊢ A ⊕ M - e
+{1, A, (P ⊸ M) & 1} ⊢ A ⊕ M  + 
+{1, A, (E ⊸ A) & 1} ⊢ A ⊕ M  +
+*)
+Qed.
+Hint Resolve aux_210 : proof.
+Hint Rewrite aux_210 : proof.
+
+Lemma aux_211 : no_proof_for ({E ⊸ A, A, P & 1, (P ⊸ M) & 1}) (A ⊕ M).
+Proof.
+  intro p;unusable_implies_tac 7%nat A p.
+Qed.
+Hint Resolve aux_211 : proof.
+
+Lemma aux_212 : no_proof_for ({E ⊸ A, P ⊸ M, A, P & 1}) (A ⊕ M).
+Proof.
+  intro p;unusable_implies_tac 7%nat A p.
+Qed.
+Hint Resolve aux_212 : proof.
+
+Lemma aux_213 : no_proof_for ({1, P ⊸ M, A, (E ⊸ A) & 1}) (A ⊕ M).
+Proof.
+  intro p;unusable_implies_tac 1%nat M p.
+Qed.
+Hint Resolve aux_213 : proof.
+
+Lemma aux_214 : no_proof_for ({1, P ⊸ M, A}) A.
+Proof.
+  intro p;unusable_implies_tac 1%nat M p.
+Qed.
+Hint Resolve aux_214 : proof.
+
+Lemma aux_215 : no_proof_for ({P ⊸ M, A, P & 1}) (A).
+Proof.
+  intros p; one_step p;eauto with proof.
+(*
+{1, P ⊸ M, A} ⊢ A
+*)
+Qed. 
+Hint Resolve aux_215 : proof.
+
+Lemma aux_216 : no_proof_for ({P ⊸ M, A, P & 1}) (A ⊕ M).
+Proof.
+  intros p; one_step p;eauto with proof.
+(*
+{P ⊸ M, A, P & 1} ⊢ A
+*)
+Qed.
+Hint Resolve aux_216 : proof.
+
+Lemma aux_217 : no_proof_for ({1, 1, P ⊸ M, A}) (A ⊕ M).
+Proof.
+  intro p;unusable_implies_tac 1%nat M p.
+Qed.
+Hint Resolve aux_217 : proof.
+
+Lemma aux_218 : no_proof_for ({1, 1, P ⊸ M, A}) A.
+Proof.
+  intro p;unusable_implies_tac 1%nat M p.
+Qed.
+Hint Resolve aux_218 : proof.
+
+Lemma aux_219 : no_proof_for ({1, P ⊸ M, A, P & 1}) A.
+Proof.
+  intros p; one_step p;eauto with proof.
+(*
+{1, 1, P ⊸ M, A} ⊢ A
+*)
+Qed.
+Hint Resolve aux_219 : proof.
+
+Lemma aux_220 : no_proof_for ({1, P ⊸ M, A, P & 1}) (A ⊕ M).
+Proof.
+  intros p; one_step p;eauto with proof.
+(*
+{P ⊸ M, A, P & 1} ⊢ A ⊕ M
+{1, 1, P ⊸ M, A} ⊢ A ⊕ M e
+{1, P ⊸ M, A, P & 1} ⊢ A
+*)
+Qed.
+Hint Resolve aux_220 : proof.
+
+Lemma aux_221 : all_proofs_of ({P ⊸ M, A, P & 1, (E ⊸ A) & 1}) (A ⊕ M).
+Proof.
+  intros p; one_step p;eauto with proof.
+(*
+{E ⊸ A, P ⊸ M, A, P & 1} ⊢ A ⊕ M  - e 
+{1, P ⊸ M, A, (E ⊸ A) & 1} ⊢ A ⊕ M - e
+{1, P ⊸ M, A, P & 1} ⊢ A ⊕ M - 
+*)
+Qed.
+Hint Resolve aux_221 : proof.
+Hint Rewrite aux_221 : proof.
+
+Lemma aux_222 : no_proof_for ({E ⊸ A, 1, A, (P ⊸ M) & 1}) (A ⊕ M).
+Proof.
+  intro p;unusable_implies_tac 7%nat A p.
+Qed.
+Hint Resolve aux_222 : proof.
+
+Lemma aux_223 : all_proofs_of ({1, 1, A, (P ⊸ M) & 1}) (A ⊕ M).
+Proof.
+  intros p; one_step p;eauto with proof.
+Qed.
+Hint Resolve aux_223 : proof.
+Hint Rewrite aux_223 : proof.
+
+Lemma aux_224 : no_proof_for ({E ⊸ A, 1, 1, A}) (A ⊕ M).
+Proof.
+  intro p;unusable_implies_tac 7%nat A p.
+Qed.
+Hint Resolve aux_224 : proof.
+
+Lemma aux_225 : all_proofs_of ({1, 1, A, (E ⊸ A) & 1}) (A ⊕ M).
+Proof.
+  intros p; one_step p;eauto with proof.
+(*
+{E ⊸ A, 1, 1, A} ⊢ A ⊕ M
+*)
+Qed.
+Hint Resolve aux_225 : proof.
+Hint Rewrite aux_225 : proof.
+
+Lemma aux_226 : all_proofs_of ({1, A, (E ⊸ A) & 1, (P ⊸ M) & 1}) (A ⊕ M).
+Proof.
+  intros p; one_step p;eauto with proof.
+(*
+{E ⊸ A, 1, A, (P ⊸ M) & 1} ⊢ A ⊕ M - e
+{1, 1, A, (P ⊸ M) & 1} ⊢ A ⊕ M     +
+{1, 1, A, (E ⊸ A) & 1} ⊢ A ⊕ M     +
+*)
+Qed.
+Hint Resolve aux_226 : proof.
+Hint Rewrite aux_226 : proof.
+
+Lemma aux_227 : all_proofs_of ({A, P & 1}) (A ⊕ M).
+Proof.
+  intros p; one_step p;eauto with proof.
+Qed.
+Hint Resolve aux_227 : proof.
+Hint Rewrite aux_227 : proof.
+
+Lemma aux_228 : all_proofs_of ({1, A, P & 1}) (A ⊕ M).
+Proof.
+  intros p; one_step p;eauto with proof.
+(*
+{A, P & 1}) (A ⊕ M)
+*)
+Qed.
+Hint Resolve aux_228 : proof.
+Hint Rewrite aux_228 : proof.
+
+Lemma aux_229 : all_proofs_of ({A, P & 1, (P ⊸ M) & 1}) (A ⊕ M).
+Proof.
+  intros p; one_step p;eauto with proof.
+(*
+   {1, A, P & 1} ⊢ A ⊕ M +
+*)
+Qed.
+Hint Resolve aux_229 : proof.
+Hint Rewrite aux_229 : proof.
+
+Lemma aux_230 : all_proofs_of ({1, 1, A, P & 1}) (A ⊕ M).
+Proof.
+  intros p; one_step p;eauto with proof.
+Qed.
+Hint Resolve aux_230 : proof.
+Hint Rewrite aux_230 : proof.
+
+Lemma aux_231 : all_proofs_of ({1, A, P & 1, (P ⊸ M) & 1}) (A ⊕ M).
+Proof.
+  intros p; one_step p;eauto with proof.
+(*
+{A, P & 1, (P ⊸ M) & 1} ⊢ A ⊕ M + 
+{1, 1, A, P & 1} ⊢ A ⊕ M +
+*)
+Qed.
+Hint Resolve aux_231 : proof.
+Hint Rewrite aux_231 : proof.
+
+Lemma aux_232 : no_proof_for ({E ⊸ A, A, P & 1}) (A ⊕ M).
+Proof.
+  intro p;unusable_implies_tac 7%nat A p.
+Qed.
+Hint Resolve aux_232 : proof.
+
+Lemma aux_233 : all_proofs_of ({A, P & 1, (E ⊸ A) & 1}) (A ⊕ M).
+Proof.
+  intros p; one_step p;eauto with proof.
+(*
+{E ⊸ A, A, P & 1} ⊢ A ⊕ M - e
+*)
+Qed.
+Hint Resolve aux_233 : proof.
+Hint Rewrite aux_233 : proof.
+
+Lemma aux_234 : no_proof_for ({E ⊸ A, 1, A, P & 1}) (A ⊕ M).
+Proof.
+  intro p;unusable_implies_tac 7%nat A p.
+Qed.
+Hint Resolve aux_234 : proof.
+
+Lemma aux_235 : all_proofs_of ({1, A, P & 1, (E ⊸ A) & 1}) (A ⊕ M).
+Proof.
+  intros p; one_step p;eauto with proof.
+(*
+ {A, P & 1, (E ⊸ A) & 1} ⊢ A ⊕ M + 
+ {E ⊸ A, 1, A, P & 1} ⊢ A ⊕ M - e
+*)
+Qed.
+Hint Resolve aux_235 : proof.
+Hint Rewrite aux_235 : proof.
+
+Lemma aux_236 : all_proofs_of ({A, P & 1, (E ⊸ A) & 1, (P ⊸ M) & 1}) (A ⊕ M).
+Proof.
+  intros p; one_step p;eauto with proof.
+(* 
+{E ⊸ A, A, P & 1, (P ⊸ M) & 1} ⊢ A ⊕ M       - e
+{P ⊸ M, A, P & 1, (E ⊸ A) & 1} ⊢ A ⊕ M       + 
+{1, A, (E ⊸ A) & 1, (P ⊸ M) & 1} ⊢ A ⊕ M     +
+{1, A, P & 1, (P ⊸ M) & 1} ⊢ A ⊕ M           +
+{1, A, P & 1, (E ⊸ A) & 1} ⊢ A ⊕ M           + 
+*)
+Qed.
+Hint Resolve aux_236 : proof.
+Hint Rewrite aux_236 : proof.
+
+Lemma aux_237 : no_proof_for ({E ⊸ A, V ⊸ A, P & 1, (P ⊸ M) & 1, V}) (A ⊕ M).
+Proof.
+  intro p;unusable_implies_tac 7%nat A p.
+Qed.
+Hint Resolve aux_237 : proof.
+
+Lemma aux_238 : no_proof_for ({V ⊸ A, P & 1, (E ⊸ A) & 1, V}) P.
+Proof.
+  intro p; unusable_var_strong_tac 5%nat 6%nat p.
+Qed.
+Hint Resolve aux_238 : proof.
+
+Lemma aux_239 : no_proof_for ({V ⊸ A, P & 1, V}) P.
+Proof.
+  intro p; unusable_var_strong_tac 5%nat 6%nat p.
+Qed.
+Hint Resolve aux_239 : proof.
+
+Lemma aux_240 : no_proof_for ({E ⊸ A, P ⊸ M, P & 1, V}) V.
+Proof.
+  intro p;unusable_implies_tac 7%nat A p.
+Qed.
+Hint Resolve aux_240 : proof.
+
+Lemma aux_241 : no_proof_for ({1, P ⊸ M, (E ⊸ A) & 1, V}) V.
+Proof.
+  intro p;unusable_implies_tac 1%nat M p.
+Qed.
+Hint Resolve aux_241 : proof.
+
+Lemma aux_242 : no_proof_for ({1, P ⊸ M, V}) V.
+Proof.
+  intro p;unusable_implies_tac 1%nat M p.
+Qed.
+Hint Resolve aux_242 : proof.
+
+Lemma aux_243 : no_proof_for ({P ⊸ M, P & 1, V}) V.
+Proof.
+  intro p;one_step p;eauto with proof.
+(*
+   {1, P ⊸ M, V} ⊢ V e
+*)
+Qed.
+Hint Resolve aux_243 : proof.
+
+Lemma aux_244 : no_proof_for ({1, 1, P ⊸ M, V}) V.
+Proof.
+  intro p;unusable_implies_tac 1%nat M p.
+Qed.
+Hint Resolve aux_244 : proof.
+
+Lemma aux_245 : no_proof_for ({1, P ⊸ M, P & 1, V}) V.
+Proof.
+  intro p;one_step p;eauto with proof.
+(*
+{P ⊸ M, P & 1, V} ⊢ V        
+{1, 1, P ⊸ M, V} ⊢ V         e 
+*)
+Qed.
+Hint Resolve aux_245 : proof.
+
+Lemma aux_246 : no_proof_for ({P ⊸ M, P & 1, (E ⊸ A) & 1, V}) V.
+Proof.
+  intros p; one_step p;eauto with proof.
+(* 
+{E ⊸ A, P ⊸ M, P & 1, V} ⊢ V     e
+{1, P ⊸ M, (E ⊸ A) & 1, V} ⊢ V   e
+{1, P ⊸ M, P & 1, V} ⊢ V          e
+*)
+Qed.
+Hint Resolve aux_246 : proof.
+Hint Rewrite aux_246 : proof.
+
+Lemma aux_247 : no_proof_for ({P ⊸ M, V}) V.
+Proof.
+  intro p;unusable_implies_tac 1%nat M p.
+Qed.
+Hint Resolve aux_247 : proof.
+
+Lemma aux_248 : no_proof_for ({P ⊸ M, (E ⊸ A) & 1, V}) V.
+Proof.
+  intro p;unusable_implies_tac 1%nat M p.
+Qed.
+Hint Resolve aux_248 : proof.
+
+Lemma aux_249 : no_proof_for ({E ⊸ A, A, P ⊸ M, P & 1}) A.
+Proof.
+  intro p;unusable_implies_tac 7%nat A p.
+Qed.
+Hint Resolve aux_249 : proof.
+
+Lemma aux_250 : no_proof_for ({1, A, P ⊸ M, (E ⊸ A) & 1}) A.
+Proof.
+  intro p;unusable_implies_tac 1%nat M p.
+Qed.
+Hint Resolve aux_250 : proof.
+
+Lemma aux_251 : no_proof_for ({A, P ⊸ M, P & 1, (E ⊸ A) & 1}) A.
+Proof.
+  intros p; one_step p;eauto with proof.
+(*
+ {E ⊸ A, A, P ⊸ M, P & 1} ⊢ A   e
+{1, A, P ⊸ M, (E ⊸ A) & 1} ⊢ A   e
+*)
+Qed.
+Hint Resolve aux_251 : proof.
+
+Lemma aux_252 : no_proof_for ({A, P ⊸ M, P & 1, (E ⊸ A) & 1}) (A ⊕ M).
+Proof.
+  intros p; one_step p;eauto with proof.
+(*
+ {A, P ⊸ M, P & 1, (E ⊸ A) & 1} ⊢ A
+*)
+Qed.
+Hint Resolve aux_252 : proof.
+
+Lemma aux_253 : no_proof_for ({E ⊸ A, P ⊸ M, V ⊸ A, P & 1, V}) (A ⊕ M).
+Proof.
+  intro p;unusable_implies_tac 7%nat A p.
+Qed.
+Hint Resolve aux_253 : proof.
+
+Lemma aux_254 : no_proof_for ({E ⊸ A, P ⊸ M, V ⊸ A, V}) (A ⊕ M).
+Proof.
+  intro p;unusable_implies_tac 7%nat A p.
+Qed.
+Hint Resolve aux_254 : proof.
+
+Lemma aux_255 : no_proof_for ({P ⊸ M, V ⊸ A, V}) A.
+Proof.
+  intro p;unusable_implies_tac 1%nat M p.
+Qed.
+Hint Resolve aux_255 : proof.
+
+Lemma aux_256 : no_proof_for ({P ⊸ M, V ⊸ A, V}) M.
+Proof.
+  intro p;unusable_var_strong_tac 5%nat 6%nat p.
+Qed.
+Hint Resolve aux_256 : proof.
+
+Lemma aux_257 : no_proof_for ({P ⊸ M, V ⊸ A, V}) (A ⊕ M).
+Proof.
+  intros p; one_step p;eauto with proof.
+(*
+{P ⊸ M, V ⊸ A, V} ⊢ A e
+{P ⊸ M, V ⊸ A, V} ⊢ M e
+*)
+Qed.
+Hint Resolve aux_257 : proof.
+
+Lemma aux_258 : no_proof_for ({1, P ⊸ M, V ⊸ A, V}) A.
+Proof.
+  intro p;unusable_implies_tac 1%nat M p.
+Qed.
+Hint Resolve aux_258 : proof.
+
+Lemma aux_259 : no_proof_for ({1, P ⊸ M, V ⊸ A, V}) M.
+Proof.
+  intro p;unusable_var_strong_tac 5%nat 6%nat p.
+Qed.
+Hint Resolve aux_259 : proof.
+
+
+Lemma aux_260 : no_proof_for ({1, P ⊸ M, V ⊸ A, V}) (A ⊕ M).
+Proof.
+  intros p; one_step p;eauto with proof.
+(*
+{P ⊸ M, V ⊸ A, V} ⊢ A ⊕ M
+{1, P ⊸ M, V ⊸ A, V} ⊢ A      e
+{1, P ⊸ M, V ⊸ A, V} ⊢ M      e
+*)
+Qed.
+Hint Resolve aux_260 : proof.
+
+Lemma aux_261 : no_proof_for ({P ⊸ M, V ⊸ A, (E ⊸ A) & 1, V}) A.
+Proof.
+  intro p;unusable_implies_tac 1%nat M p.
+Qed.
+Hint Resolve aux_261 : proof.
+
+Lemma aux_262 : no_proof_for ({P ⊸ M, V ⊸ A, (E ⊸ A) & 1, V}) M.
+Proof.
+  intro p;unusable_var_strong_tac 5%nat 6%nat p.
+Qed.
+Hint Resolve aux_262 : proof.
+
+Lemma aux_263 : no_proof_for ({P ⊸ M, V ⊸ A, (E ⊸ A) & 1, V}) (A ⊕ M).
+Proof.
+  intros p; one_step p;eauto with proof.
+(*
+{E ⊸ A, P ⊸ M, V ⊸ A, V} ⊢ A ⊕ M  e
+{1, P ⊸ M, V ⊸ A, V} ⊢ A ⊕ M 
+{P ⊸ M, V ⊸ A, (E ⊸ A) & 1, V} ⊢ A  e
+{P ⊸ M, V ⊸ A, (E ⊸ A) & 1, V} ⊢ M  e
+*)
+Qed.
+Hint Resolve aux_263 : proof.
+
+Lemma aux_264 : no_proof_for ({E ⊸ A, 1, P ⊸ M, V ⊸ A, V}) (A ⊕ M).
+Proof.
+  intro p;unusable_implies_tac 7%nat A p.
+Qed.
+Hint Resolve aux_264 : proof.
+
+Lemma aux_265 : no_proof_for ({1, 1, P ⊸ M, V ⊸ A, V}) A.
+Proof.
+  intro p;unusable_implies_tac 1%nat M p.
+Qed.
+Hint Resolve aux_265 : proof.
+
+Lemma aux_266 : no_proof_for ({1, 1, P ⊸ M, V ⊸ A, V}) M.
+Proof.
+  intro p;unusable_var_strong_tac 5%nat 6%nat p.
+Qed.
+Hint Resolve aux_266 : proof.
+
+Lemma aux_267 : no_proof_for ({1, 1, P ⊸ M, V ⊸ A, V}) (A ⊕ M).
+Proof.
+  intros p; one_step p;eauto with proof.
+(*
+{1, 1, P ⊸ M, V ⊸ A, V} ⊢ A  e
+{1, 1, P ⊸ M, V ⊸ A, V} ⊢ M  e
+*)
+Qed.
+Hint Resolve aux_267 : proof.
+
+Lemma aux_268 : no_proof_for ({1, P ⊸ M, V ⊸ A, (E ⊸ A) & 1, V}) A.
+Proof.
+  intro p;unusable_implies_tac 1%nat M p.
+Qed.
+Hint Resolve aux_268 : proof.
+
+Lemma aux_269 : no_proof_for ({1, P ⊸ M, V ⊸ A, (E ⊸ A) & 1, V}) M.
+Proof.
+  intro p;unusable_var_strong_tac 5%nat 6%nat p.
+Qed.
+Hint Resolve aux_269 : proof.
+
+Lemma aux_270 : no_proof_for ({1, P ⊸ M, V ⊸ A, (E ⊸ A) & 1, V}) (A ⊕ M).
+Proof.
+  intros p; one_step p;eauto with proof.
+(*
+{P ⊸ M, V ⊸ A, (E ⊸ A) & 1, V} ⊢ A ⊕ M
+{E ⊸ A, 1, P ⊸ M, V ⊸ A, V} ⊢ A ⊕ M        e
+{1, 1, P ⊸ M, V ⊸ A, V} ⊢ A ⊕ M
+{1, P ⊸ M, V ⊸ A, (E ⊸ A) & 1, V} ⊢ A      e
+{1, P ⊸ M, V ⊸ A, (E ⊸ A) & 1, V} ⊢ M      e
+*)
+Qed.
+Hint Resolve aux_270 : proof.
+
+Lemma aux_271 : no_proof_for ({1, P ⊸ M, V ⊸ A, P & 1, V}) (A ⊕ M).
+Proof.
+  intros p; one_step p;eauto with proof.
+*****
+(*
+*{1, V ⊸ A, P & 1, V} ⊢ P   e
+{P ⊸ M, V ⊸ A, P & 1, V} ⊢ A ⊕ M
+{1, P ⊸ M, V ⊸ A, P & 1, V} ⊢ A 
+{1, P ⊸ M, V ⊸ A, P & 1, V} ⊢ M  e
+*)
+Qed.
+Hint Resolve aux_270 : proof.
+
+Lemma aux_238 : no_proof_for ({P ⊸ M, V ⊸ A, P & 1, (E ⊸ A) & 1, V}) (A ⊕ M).
+Proof.
+  intros p; one_step p;eauto with proof.
+(*
+{V ⊸ A, P & 1, (E ⊸ A) & 1, V} ⊢ P              e
+{V ⊸ A, P & 1, V} ⊢ P                           e 
+{P ⊸ M, P & 1, (E ⊸ A) & 1, V} ⊢ V
+{P ⊸ M, P & 1, V} ⊢ V
+{P ⊸ M, V} ⊢ V                                  e
+{P ⊸ M, (E ⊸ A) & 1, V} ⊢ V                     e
+{A, P ⊸ M, P & 1, (E ⊸ A) & 1} ⊢ A ⊕ M
+{E ⊸ A, P ⊸ M, V ⊸ A, P & 1, V} ⊢ A ⊕ M        e
+{1, P ⊸ M, V ⊸ A, (E ⊸ A) & 1, V} ⊢ A ⊕ M
+*{1, P ⊸ M, V ⊸ A, P & 1, V} ⊢ A ⊕ M
+{P ⊸ M, V ⊸ A, P & 1, (E ⊸ A) & 1, V} ⊢ A      e
+{P ⊸ M, V ⊸ A, P & 1, (E ⊸ A) & 1, V} ⊢ M      e
+*)
+Qed.
+Hint Resolve aux_235 : proof.
+Hint Rewrite aux_235 : proof.
+
+Lemma aux_112 : all_proofs_of ({V ⊸ A, P & 1, (E ⊸ A) & 1, (P ⊸ M) & 1, V}) (A ⊕ M).
+Proof.
+  intros p; one_step p;eauto with proof.
+(*
+{A, (P ⊸ M) & 1} ⊢ A ⊕ M                      +
+{A, (E ⊸ A) & 1, (P ⊸ M) & 1} ⊢ A ⊕ M           +
+{A, (E ⊸ A) & 1} ⊢ A ⊕ M                        + 
+{A, P & 1, (E ⊸ A) & 1, (P ⊸ M) & 1} ⊢ A ⊕ M    +
+{A, P & 1, (E ⊸ A) & 1} ⊢ A ⊕ M                  +
+{A, P & 1} ⊢ A ⊕ M                               +
+{A, P & 1, (P ⊸ M) & 1} ⊢ A ⊕ M                  +
+{E ⊸ A, V ⊸ A, P & 1, (P ⊸ M) & 1, V} ⊢ A ⊕ M   - e
+*{P ⊸ M, V ⊸ A, P & 1, (E ⊸ A) & 1, V} ⊢ A ⊕ M   - 
+{1, V ⊸ A, (E ⊸ A) & 1, (P ⊸ M) & 1, V} ⊢ A ⊕ M +
+{1, V ⊸ A, P & 1, (P ⊸ M) & 1, V} ⊢ A ⊕ M       +
+{1, V ⊸ A, P & 1, (E ⊸ A) & 1, V} ⊢ A ⊕ M       +
+{V ⊸ A, P & 1, (E ⊸ A) & 1, (P ⊸ M) & 1, V} ⊢ M - e
+*)
+Qed.
+Hint Resolve aux_112 : proof.
+Hint Rewrite aux_112 : proof. 
+*)
+
+Lemma aux_1 : all_proofs_of ({A}) (A ⊕ M).
+Proof.
+  intros p; one_step p;eauto with proof.
+Qed.
+Hint Resolve aux_1 : proof.
+Hint Rewrite aux_1 : proof.
+
+Lemma proof_1 : all_proofs_of ({ (V⊸A),V}) (A⊕M).
+Proof.
+  intros p; one_step p;eauto with proof.
 Qed.
 Hint Resolve proof_1 : proof.
 Hint Rewrite proof_1 : proof.
 
-Lemma proof_aux_2 : all_proof_of ({V} ⊢ A ⊕ M).
+Lemma proof_2 : all_proofs_of ({(V⊸A)&1, V}) (A⊕M).
 Proof.
-  intros p.
-  one_step p.
-Qed.
-Hint Resolve proof_aux_2 : proof.
-Hint Rewrite proof_aux_2 : proof.
-
-Lemma proof_aux_3 : all_proof_of ({1, V} ⊢ A ⊕ M).
-Proof.
-  intros p.
-  one_step p.
-Qed.
-Hint Resolve proof_aux_3 : proof.
-Hint Rewrite proof_aux_3 : proof.
-
-Lemma proof_aux_4 : all_proof_of ({(V ⊸ A) & 1, V} ⊢ M).
-Proof.
-  intros p.
-  one_step p.
-Qed.
-Hint Resolve proof_aux_4 : proof.
-Hint Rewrite proof_aux_4 : proof.
-
-Lemma proof_2 : forall (p:{(V⊸A)&1, V}⊢A⊕M), 
-  exists_AtheseA_on_formula (fun _ _ _ => trueP) A M _ _ p  = trueP.
-Proof.
-  intros p.
-  one_step p.
+  intros p;one_step p;eauto with proof.
 Qed.
 Hint Resolve proof_2 : proof.
 Hint Rewrite proof_2 : proof.
 
-Lemma proof_aux_5 : all_proof_of ( {A,1} ⊢ A ⊕ M).
+Lemma aux_2 : all_proofs_of ({A, 1}) (A ⊕ M).
 Proof.
-  intros p.
-  one_step p.
+  intros p; one_step p;eauto with proof.
 Qed.
-Hint Resolve proof_aux_5 : proof.
-Hint Rewrite proof_aux_5 : proof.
+Hint Resolve aux_2 : proof.
+Hint Rewrite aux_2 : proof.
 
-Lemma proof_aux_6 : all_proof_of ( { (V ⊸ A), 1,V} ⊢ A ⊕ M).
+Lemma aux_3 : all_proofs_of ({V ⊸ A, 1, V})  (A ⊕ M).
 Proof.
-  intros p.
-  one_step p.
-  decompose_union;repeat tutu;finish.
+  intros p; one_step p;eauto with proof.
 Qed.
-Hint Resolve proof_aux_6 : proof.
-Hint Rewrite proof_aux_6 : proof.
+Hint Resolve aux_3 : proof.
+Hint Rewrite aux_3 : proof.
 
-Lemma proof_aux_7 : all_proof_of ({1, 1, V} ⊢ A ⊕ M).
+Lemma aux_4 : all_proofs_of ({1, (V ⊸ A) & 1, V}) (A ⊕ M).
 Proof.
-  intros p;one_step p.
+  intros p; one_step p;eauto with proof.
 Qed.
-Hint Resolve proof_aux_7 : proof.
-Hint Rewrite proof_aux_7 : proof.
+Hint Resolve aux_4 : proof.
+Hint Rewrite aux_4 : proof.
 
-Lemma proof_aux_8 : all_proof_of ( {1, (V ⊸ A) & 1, V} ⊢ A ⊕ M).
+Lemma aux_5 : all_proofs_of ({A, 1, 1}) (A ⊕ M).
 Proof.
-  intros p.
-  one_step p.
+  intros p; one_step p;eauto with proof.
 Qed.
-Hint Resolve proof_aux_8 : proof.
-Hint Rewrite proof_aux_8 : proof.
+Hint Resolve aux_5 : proof.
+Hint Rewrite aux_5 : proof.
 
-
-Lemma proof_aux_9 : all_proof_of ( {A, 1, 1} ⊢ A ⊕ M).
+Lemma aux_6 : all_proofs_of ({V ⊸ A, 1, 1, V}) (A ⊕ M).
 Proof.
-  intros p.
-  one_step p.
+  intros p; one_step p;eauto with proof.
 Qed.
-Hint Resolve proof_aux_9 : proof.
-Hint Rewrite proof_aux_9 : proof.
+Hint Resolve aux_6 : proof.
+Hint Rewrite aux_6 : proof.
 
-
-Lemma proof_aux_10 : all_proof_of ( {V ⊸ A, 1, 1, V} ⊢ A ⊕ M).
+Lemma aux_7 : all_proofs_of ({1, 1, (V ⊸ A) & 1, V}) (A ⊕ M).
 Proof.
-  intros p.
-  one_step p.
-  decompose_union;repeat tutu;finish.
+  intros p; one_step p;eauto with proof.
 Qed.
-Hint Resolve proof_aux_10 : proof.
-Hint Rewrite proof_aux_10: proof.
+Hint Resolve aux_7 : proof.
+Hint Rewrite aux_7 : proof.
 
-Lemma proof_aux_11 : all_proof_of ({1, 1, 1, V} ⊢ A ⊕ M).
+Lemma aux_8 : all_proofs_of ({A, 1, 1, 1}) (A ⊕ M).
 Proof.
-  intros p;one_step p.
+  intros p; one_step p;eauto with proof.
 Qed.
-Hint Resolve proof_aux_11 : proof.
-Hint Rewrite proof_aux_11: proof.
+Hint Resolve aux_8 : proof.
+Hint Rewrite aux_8 : proof.
 
-Lemma proof_aux_12 : all_proof_of ({1, 1, (V ⊸ A) & 1, V} ⊢ A ⊕ M).
+Lemma aux_9 : all_proofs_of ({V ⊸ A, 1, 1, 1, V}) (A ⊕ M).
 Proof.
-  intros p.
-  one_step p.
+  intros p; one_step p;eauto with proof.
 Qed.
-Hint Resolve proof_aux_12 : proof.
-Hint Rewrite proof_aux_12: proof.
+Hint Resolve aux_9 : proof.
+Hint Rewrite aux_9 : proof.
 
-Lemma proof_aux_13 : all_proof_of ({1, 1, 1, V} ⊢ A ⊕ M).
+Lemma proof_3 : all_proofs_of ({1,1,1,(V⊸A)&1, V}) (A⊕M).
 Proof.
-  intros p.
-  one_step p.
+  intros p; one_step p;eauto with proof.
 Qed.
-Hint Resolve proof_aux_13 : proof.
-Hint Rewrite proof_aux_13: proof.
+Hint Resolve proof_3 : proof.
+Hint Rewrite proof_3 : proof.
 
-Lemma proof_aux_14 : all_proof_of ({A,1, 1, 1} ⊢ A ⊕ M).
+Lemma aux_17 : no_proof_for ({P, (E ⊸ A) & 1, (P ⊸ M) & 1, V}) V.
 Proof.
-  intros p.
-  one_step p.
+  intro p; unusable_var_strong_tac 1%nat 8%nat p.
 Qed.
-Hint Resolve proof_aux_14 : proof.
-Hint Rewrite proof_aux_14: proof.
-
-Lemma proof_aux_15 : all_proof_of ({V ⊸ A, 1, 1, 1, V} ⊢ A ⊕ M).
+Hint Resolve aux_17 : proof.
+Lemma aux_15 : no_proof_for ({P, (P ⊸ M) & 1, V}) V.
 Proof.
-  intros p.
-  one_step p.
-  decompose_union;repeat tutu;try finish.
+  intro p; unusable_var_strong_tac 1%nat 8%nat p.
 Qed.
-Hint Resolve proof_aux_15 : proof.
-Hint Rewrite proof_aux_15: proof.
+Hint Resolve aux_15 : proof.
 
-Lemma proof_aux_16 : all_proof_of ({1, 1, 1, 1, V} ⊢ A ⊕ M).
+Lemma aux_18 : no_proof_for ({E ⊸ A, A, P, (P ⊸ M) & 1}) (A ⊕ M).
 Proof.
-  intros p.
-  one_step p.
+  intro p;unusable_implies_tac 7%nat A p.
 Qed.
-Hint Resolve proof_aux_16 : proof.
-Hint Rewrite proof_aux_16: proof.
+Hint Resolve aux_18 : proof.
 
-
-Lemma proof_3 : all_proof_of ({1,1,1,(V⊸A)&1, V}⊢A⊕M).
+Lemma aux_19 : no_proof_for ({M, A}) (A ⊕ M).
 Proof.
-  intros p.
-  one_step p.
+  intros p; one_step p;eauto with proof.
 Qed.
+Hint Resolve aux_19 : proof.
+
+Lemma aux_20 : no_proof_for ({E ⊸ A, M, A}) (A ⊕ M).
+Proof.
+  intro p;unusable_implies_tac 7%nat A p.
+Qed.
+Hint Resolve aux_20 : proof.
+
+Lemma aux_21 : no_proof_for ({1, M, A})(A ⊕ M).
+Proof.
+  intros p; one_step p;eauto with proof.
+Qed.
+Hint Resolve aux_21 : proof.
+
+Lemma aux_22 : no_proof_for ({M, A, (E ⊸ A) & 1}) (A ⊕ M).
+Proof.
+  intros p; one_step p;eauto with proof.
+(*
+   {E ⊸ A, M, A} ⊢ A ⊕ M
+   {1, M, A} ⊢ A ⊕ M
+*)
+Qed.
+Hint Resolve aux_22 : proof.
+
+Lemma aux_23 : no_proof_for ({E ⊸ A, P ⊸ M, A, P}) (A ⊕ M).
+Proof.
+  intro p;unusable_implies_tac 7%nat A p.
+Qed.
+Hint Resolve aux_23 : proof.
+
+Lemma aux_24 : no_proof_for ({P ⊸ M, A, P}) A.
+Proof.
+  intro p.
+  unusable_var_strong_tac 1%nat 8%nat p.
+Qed.
+Hint Resolve aux_24 : proof.
+
+Lemma aux_25 : no_proof_for ({P ⊸ M, A, P}) (A ⊕ M).
+Proof.
+  intros p; one_step p;eauto with proof.
+(*
+   {P ⊸ M, A, P} ⊢ A
+*)
+Qed.
+Hint Resolve aux_25 : proof.
+
+Lemma aux_26 : no_proof_for ({1, P ⊸ M, A, P}) A.
+Proof.
+  intro p.
+  unusable_var_strong_tac 1%nat 8%nat p.
+Qed.
+Hint Resolve aux_26 : proof.
+
+Lemma aux_27 : no_proof_for ({1, P ⊸ M, A, P}) (A ⊕ M).
+Proof.
+  intros p; one_step p;eauto with proof.
+(* 
+   {P ⊸ M, A, P} ⊢ A ⊕ M
+   {1, P ⊸ M, A, P} ⊢ A 
+*)
+Qed.
+Hint Resolve aux_27 : proof.
+
+Lemma aux_29 : no_proof_for ({P ⊸ M, A, P, (E ⊸ A) & 1}) A.
+Proof.
+  intro p.
+  unusable_var_strong_tac 1%nat 8%nat p.
+Qed.
+Hint Resolve aux_29 : proof.
+
+Lemma aux_30 : no_proof_for ({P ⊸ M, A, P, (E ⊸ A) & 1}) (A ⊕ M).
+Proof.
+  intros p; one_step p;eauto with proof.
+(*
+{M, A} ⊢ A ⊕ M
+{M, A, (E ⊸ A) & 1} ⊢ A ⊕ M
+{E ⊸ A, P ⊸ M, A, P} ⊢ A ⊕ M
+{1, P ⊸ M, A, P} ⊢ A ⊕ M
+{P ⊸ M, A, P, (E ⊸ A) & 1} ⊢ A e
+*)
+Qed.
+Hint Resolve aux_30 : proof.
+
+Lemma aux_31 : no_proof_for ({A, P, (P ⊸ M) & 1}) A.
+Proof.
+  intros p; unusable_var_strong_tac 1%nat 8%nat p.
+Qed.
+Hint Resolve aux_31 : proof.
+
+Lemma aux_32 : no_proof_for ({A, P, (P ⊸ M) & 1}) (A ⊕ M).
+Proof.
+  intros p; one_step p;eauto with proof.
+(* 
+   ({A, P, (P ⊸ M) & 1}) A
+*)
+Qed.
+Hint Resolve aux_32 : proof.
+
+Lemma aux_33 : no_proof_for ({1, A, P, (P ⊸ M) & 1}) A.
+Proof.
+  intros p; unusable_var_strong_tac 1%nat 8%nat p.
+Qed.
+Hint Resolve aux_33 : proof.
+
+Lemma aux_34 : no_proof_for ({1, A, P, (P ⊸ M) & 1}) (A ⊕ M).
+Proof.
+  intros p; one_step p;eauto with proof.
+(*
+ {A, P, (P ⊸ M) & 1} ⊢ A ⊕ M
+ {1, A, P, (P ⊸ M) & 1} ⊢ A
+*)
+Qed.
+Hint Resolve aux_34 : proof.
+
+Lemma aux_36 : no_proof_for ({A, P, (E ⊸ A) & 1, (P ⊸ M) & 1}) A.
+Proof.
+  intros p; unusable_var_strong_tac 1%nat 8%nat p.
+Qed.
+Hint Resolve aux_36 : proof.
+
+Lemma aux_37 : no_proof_for ({A, P, (E ⊸ A) & 1, (P ⊸ M) & 1}) (A ⊕ M).
+Proof.
+  intros p; one_step p;eauto with proof.
+(*
+{E ⊸ A, A, P, (P ⊸ M) & 1} ⊢ A ⊕ M
+{P ⊸ M, A, P, (E ⊸ A) & 1} ⊢ A ⊕ M  
+{1, A, P, (P ⊸ M) & 1} ⊢ A ⊕ M
+{A, P, (E ⊸ A) & 1, (P ⊸ M) & 1} ⊢ A
+*)
+Qed.
+Hint Resolve aux_37 : proof.
+
+Lemma aux_42 : no_proof_for ({V ⊸ A, P, (E ⊸ A) & 1, V}) P.
+Proof.
+  intro p.
+  unusable_var_strong_tac 5%nat 6%nat p.
+Qed.
+Hint Resolve aux_42 : proof.
+
+Lemma aux_40 : no_proof_for ({V ⊸ A, P, V}) P.
+Proof.
+  intro p.
+  unusable_var_strong_tac 5%nat 6%nat p.
+Qed.
+Hint Resolve aux_40 : proof.
+
+Lemma aux_43 : no_proof_for ({M, V ⊸ A, V}) M.
+Proof.
+  intro p.
+  unusable_var_strong_tac 5%nat 6%nat p.
+Qed.
+Hint Resolve aux_43 : proof.
+
+Lemma aux_44 : no_proof_for ({M, V ⊸ A, V}) (A ⊕ M).
+Proof.
+  intros p; one_step p;eauto with proof.
+(* 
+   {M, V ⊸ A, V} ⊢ M
+*)
+Qed.
+Hint Resolve aux_44 : proof.
+
+Lemma aux_45 : no_proof_for ({E ⊸ A, M, V ⊸ A, V}) (A ⊕ M).
+Proof.
+  intro p;unusable_implies_tac 7%nat A p.
+Qed.
+Hint Resolve aux_45 : proof.
+
+Lemma aux_46 : no_proof_for ({1, M, V ⊸ A, V}) (M).
+Proof.
+  intro p.
+  unusable_var_strong_tac 5%nat 6%nat p.
+Qed.
+Hint Resolve aux_46 : proof.
+
+Lemma aux_47 : no_proof_for ({1, M, V ⊸ A, V}) (A ⊕ M).
+Proof.
+  intros p; one_step p;eauto with proof.
+(*
+{1, M, V ⊸ A, V} ⊢ M
+*)
+Qed.
+Hint Resolve aux_47 : proof.
+
+Lemma aux_49 : no_proof_for ({M, V ⊸ A, (E ⊸ A) & 1, V}) M.
+Proof.
+  intro p.
+  unusable_var_strong_tac 5%nat 6%nat p.
+Qed.
+Hint Resolve aux_49 : proof.
+
+
+Lemma aux_50 : no_proof_for ({M, V ⊸ A, (E ⊸ A) & 1, V}) (A ⊕ M).
+Proof.
+  intros p; one_step p;eauto with proof.
+(*
+ {E ⊸ A, M, V ⊸ A, V} ⊢ A ⊕ M
+ {1, M, V ⊸ A, V} ⊢ A ⊕ M
+ {M, V ⊸ A, (E ⊸ A) & 1, V} ⊢ M 
+*)
+Qed.
+Hint Resolve aux_50 : proof.
+
+Lemma aux_51 : no_proof_for ({E ⊸ A, P ⊸ M, V ⊸ A, P, V}) (A ⊕ M).
+Proof.
+  intro p;unusable_implies_tac 7%nat A p.
+Qed.
+Hint Resolve aux_51 : proof.
+
+Lemma aux_41 : no_proof_for ({1, V ⊸ A, P, V}) P.
+Proof.
+  intro p.
+  unusable_var_strong_tac 5%nat 6%nat p.
+Qed.
+Hint Resolve aux_41 : proof.
+
+
+Lemma aux_52 : no_proof_for ({P ⊸ M, V ⊸ A, P, V}) A.
+Proof.
+  intro p.
+  unusable_var_strong_tac 1%nat 8%nat p.
+Qed.
+Hint Resolve aux_52 : proof.
+
+Lemma aux_53 : no_proof_for ({P ⊸ M, V ⊸ A, P, V}) M.
+Proof.
+  intro p.
+  unusable_var_strong_tac 5%nat 6%nat p.
+Qed.
+Hint Resolve aux_53 : proof.
+
+Lemma aux_12 : no_proof_for ({P ⊸ M, P, V}) V.
+Proof.
+  intro p.
+  unusable_var_strong_tac 1%nat 8%nat p.
+Qed.
+Hint Resolve aux_12 : proof.
+
+Lemma aux_54 : no_proof_for ({P ⊸ M, V ⊸ A, P, V}) (A ⊕ M).
+Proof.
+  intros p; one_step p;eauto with proof.
+(*
+   {P ⊸ M, P, V} ⊢ V
+   {P ⊸ M, V ⊸ A, P, V} ⊢ A
+   {P ⊸ M, V ⊸ A, P, V} ⊢ M
+*)
+Qed.
+Hint Resolve aux_54 : proof.
+
+Lemma aux_55 : no_proof_for ({1, P ⊸ M, V ⊸ A, P, V}) A.
+Proof.
+  intro p.
+  unusable_var_strong_tac 1%nat 8%nat p.
+Qed.
+Hint Resolve aux_55 : proof.
+
+Lemma aux_56 : no_proof_for ({1, P ⊸ M, V ⊸ A, P, V}) M.
+Proof.
+  intro p.
+  unusable_var_strong_tac 5%nat 6%nat p.
+Qed.
+Hint Resolve aux_56 : proof.
+
+Lemma aux_13 : no_proof_for ({1, P ⊸ M, P, V}) V.
+Proof.
+  intro p.
+  unusable_var_strong_tac 1%nat 8%nat p.
+Qed.
+Hint Resolve aux_13 : proof.
+
+
+Lemma aux_57 : no_proof_for  ({1, P ⊸ M, V ⊸ A, P, V}) (A ⊕ M).
+Proof.
+  intros p; one_step p;eauto with proof.
+(*
+{1, V ⊸ A, P, V} ⊢ P 
+{P ⊸ M, V ⊸ A, P, V} ⊢ A ⊕ M
+{1, P ⊸ M, V ⊸ A, P, V} ⊢ A 
+{1, P ⊸ M, V ⊸ A, P, V} ⊢ M
+{1, P ⊸ M, P, V} ⊢ V
+*)
+Qed.
+Hint Resolve aux_57 : proof.
+
+Lemma aux_59 : no_proof_for ({P ⊸ M, V ⊸ A, P, (E ⊸ A) & 1, V}) A.
+Proof.
+  intro p.
+  unusable_var_strong_tac 1%nat 8%nat p.
+Qed.
+Hint Resolve aux_59 : proof.
+
+Lemma aux_60 : no_proof_for ({E ⊸ A, P ⊸ M, V ⊸ A, P, V}) M.
+Proof.
+  intro p;unusable_implies_tac 7%nat A p.
+Qed.
+Hint Resolve aux_60 : proof.
+
+Lemma aux_14 : no_proof_for ({P ⊸ M, P, (E ⊸ A) & 1, V}) V.
+Proof.
+  intro p.
+  unusable_var_strong_tac 1%nat 8%nat p.
+Qed.
+Hint Resolve aux_14 : proof.
+
+Lemma aux_61 : no_proof_for ({P ⊸ M, V ⊸ A, P, (E ⊸ A) & 1, V}) M.
+Proof.
+  intro p.
+  unusable_var_strong_tac 5%nat 6%nat p.
+Qed.
+Hint Resolve aux_61 : proof.
+
+Lemma aux_62 : no_proof_for ({P ⊸ M, V ⊸ A, P, (E ⊸ A) & 1, V}) (A ⊕ M).
+Proof.
+  intros p; one_step p;eauto with proof.
+(*
+ {V ⊸ A, P, (E ⊸ A) & 1, V} ⊢ P e
+ {V ⊸ A, P, V} ⊢ P e
+ {M, V ⊸ A, V} ⊢ A ⊕ M
+ {M, V ⊸ A, (E ⊸ A) & 1, V} ⊢ A ⊕ M
+ {E ⊸ A, P ⊸ M, V ⊸ A, P, V} ⊢ A ⊕ M
+ {1, P ⊸ M, V ⊸ A, P, V} ⊢ A ⊕ M
+ {P ⊸ M, V ⊸ A, P, (E ⊸ A) & 1, V} ⊢ A e
+ {P ⊸ M, V ⊸ A, P, (E ⊸ A) & 1, V} ⊢ M e
+ {P ⊸ M, P, (E ⊸ A) & 1, V} ⊢ V
+ {P ⊸ M, V ⊸ A, P, (E ⊸ A) & 1, V} ⊢ M
+ *)
+Qed.
+Hint Resolve aux_62 : proof.
+
+
+Lemma aux_38 : no_proof_for ({E ⊸ A, V ⊸ A, P, (P ⊸ M) & 1, V}) (A ⊕ M).
+Proof.
+  intro p;unusable_implies_tac 7%nat A p.
+Qed.
+Hint Resolve aux_38 : proof.
+
+Lemma aux_63 : no_proof_for ({V ⊸ A, P, (P ⊸ M) & 1, V}) A.
+Proof.
+  intros p; unusable_var_strong_tac 1%nat 8%nat p.
+Qed.
+Hint Resolve aux_63 : proof.
+
+Lemma aux_64 : no_proof_for ({V ⊸ A, P, (P ⊸ M) & 1, V}) M.
+Proof.
+  intro p.
+  unusable_var_strong_tac 5%nat 6%nat p.
+Qed.
+Hint Resolve aux_64 : proof.
+
+Lemma aux_65 : no_proof_for ({V ⊸ A, P, (P ⊸ M) & 1, V}) (A ⊕ M).
+Proof.
+  intros p; one_step p;eauto with proof.
+(*
+ {V ⊸ A, P, (P ⊸ M) & 1, V} ⊢ A
+ {V ⊸ A, P, (P ⊸ M) & 1, V} ⊢ M e
+*)
+Qed.
+Hint Resolve aux_65 : proof.
+
+Lemma aux_66 : no_proof_for ({1, V ⊸ A, P, (P ⊸ M) & 1, V}) A.
+Proof.
+  intros p; unusable_var_strong_tac 1%nat 8%nat p.
+Qed.
+Hint Resolve aux_66 : proof.
+
+Lemma aux_67 : no_proof_for ({1, V ⊸ A, P, (P ⊸ M) & 1, V}) M.
+Proof.
+  intro p.
+  unusable_var_strong_tac 5%nat 6%nat p.
+Qed.
+Hint Resolve aux_67 : proof.
+
+Lemma aux_16 : no_proof_for ({1, P, (P ⊸ M) & 1, V}) V.
+Proof.
+  intros p; unusable_var_strong_tac 1%nat 8%nat p.
+Qed.
+Hint Resolve aux_16 : proof.
+
+Lemma aux_68 : no_proof_for ({1, V ⊸ A, P, (P ⊸ M) & 1, V}) (A ⊕ M).
+Proof.
+  intros p; one_step p;eauto with proof.
+(*
+ {V ⊸ A, P, (P ⊸ M) & 1, V} ⊢ A ⊕ M
+ {1, V ⊸ A, P, (P ⊸ M) & 1, V} ⊢ A
+ {1, V ⊸ A, P, (P ⊸ M) & 1, V} ⊢ M e
+ {1, P, (P ⊸ M) & 1, V} ⊢ V
+*)
+Qed.
+Hint Resolve aux_68 : proof.
+
+Lemma aux_70 : no_proof_for ({V ⊸ A, P, (E ⊸ A) & 1, (P ⊸ M) & 1, V}) A.
+Proof.
+  intros p; unusable_var_strong_tac 1%nat 8%nat p.
+Qed.
+Hint Resolve aux_70 : proof.
+
+Lemma aux_72 : no_proof_for ({V ⊸ A, P, (E ⊸ A) & 1, (P ⊸ M) & 1, V}) M.
+Proof.
+  intro p.
+  unusable_var_strong_tac 5%nat 6%nat p.
+Qed.
+Hint Resolve aux_72 : proof.
+
+Lemma aux_73 : no_proof_for ({V ⊸ A, P, (E ⊸ A) & 1, (P ⊸ M) & 1, V}) (A ⊕ M).
+Proof.
+  intros p; one_step p;eauto with proof.
+(*
+{P, (E ⊸ A) & 1, (P ⊸ M) & 1, V} ⊢ V           
+{P, (P ⊸ M) & 1, V} ⊢ V                       
+{A, P, (E ⊸ A) & 1, (P ⊸ M) & 1} ⊢ A ⊕ M
+{A, P, (P ⊸ M) & 1} ⊢ A ⊕ M
+{P ⊸ M, V ⊸ A, P, (E ⊸ A) & 1, V} ⊢ A ⊕ M
+{E ⊸ A, V ⊸ A, P, (P ⊸ M) & 1, V} ⊢ A ⊕ M
+{1, V ⊸ A, P, (P ⊸ M) & 1, V} ⊢ A ⊕ M
+{V ⊸ A, P, (E ⊸ A) & 1, (P ⊸ M) & 1, V} ⊢ A
+{V ⊸ A, P, (E ⊸ A) & 1, (P ⊸ M) & 1, V} ⊢ M    e 
+*)
+Qed.
+Hint Resolve aux_73 : proof.
+
+Lemma aux_74 : no_proof_for ({E ⊸ A, P, (V ⊸ A) & 1, (P ⊸ M) & 1, V}) (A ⊕ M).
+Proof.
+  intro p;unusable_implies_tac 7%nat A p.
+Qed.
+Hint Resolve aux_74 : proof.
+
+Lemma aux_78 : no_proof_for ({P, (V ⊸ A) & 1, (E ⊸ A) & 1, V}) P.
+Proof.
+  intros p; unusable_var_strong_tac 5%nat 6%nat p.
+Qed.
+Hint Resolve aux_78 : proof.
+
+Lemma aux_76 : no_proof_for ({P, (V ⊸ A) & 1, V}) P.
+Proof.
+  intros p; unusable_var_strong_tac 5%nat 6%nat p.
+Qed.
+Hint Resolve aux_76 : proof.
+
+Lemma aux_79 : no_proof_for ({E ⊸ A, M, (V ⊸ A) & 1, V}) (A ⊕ M).
+Proof.
+  intro p;unusable_implies_tac 7%nat A p.
+Qed.
+Hint Resolve aux_79 : proof.
+
+Lemma aux_80 : no_proof_for ({M, (V ⊸ A) & 1, V}) (M).
+Proof.
+  intros p;  unusable_var_strong_tac 5%nat 6%nat p.
+Qed.
+Hint Resolve aux_80 : proof.
+
+Lemma aux_88 : no_proof_for ({M, (V ⊸ A) & 1, V}) (A ⊕ M).
+Proof.
+  intros p; one_step p;eauto with proof.
+(*
+*   {M, (V ⊸ A) & 1, V} ⊢ M
+*)
+Qed.
+Hint Resolve aux_88 : proof.
+
+Lemma aux_82 : no_proof_for ({1, M, (V ⊸ A) & 1, V}) M.
+Proof.
+  intros p; unusable_var_strong_tac 5%nat 6%nat p.
+Qed.
+Hint Resolve aux_82 : proof.
+
+Lemma aux_83 : no_proof_for ({1, M, (V ⊸ A) & 1, V}) (A ⊕ M).
+Proof.
+  intros p; one_step p;eauto with proof.
+(*
+{M, (V ⊸ A) & 1, V} ⊢ A ⊕ M
+ {1, M, (V ⊸ A) & 1, V} ⊢ M
+*)
+Qed.
+Hint Resolve aux_83 : proof.
+
+Lemma aux_85 : no_proof_for ({M, (V ⊸ A) & 1, (E ⊸ A) & 1, V}) M.
+Proof.
+  intros p; unusable_var_strong_tac 5%nat 6%nat p.
+Qed.
+Hint Resolve aux_85 : proof.
+
+Lemma aux_86 : no_proof_for ({M, (V ⊸ A) & 1, (E ⊸ A) & 1, V}) (A ⊕ M).
+Proof.
+  intros p; one_step p;eauto with proof.
+(*
+{E ⊸ A, M, (V ⊸ A) & 1, V} ⊢ A ⊕M 
+{1, M, (V ⊸ A) & 1, V} ⊢ A ⊕ M
+{M, (V ⊸ A) & 1, (E ⊸ A) & 1, V} ⊢ M
+*)
+Qed.
+Hint Resolve aux_86 : proof.
+
+Lemma aux_89 : no_proof_for ({E ⊸ A, P ⊸ M, P, (V ⊸ A) & 1, V}) (A ⊕ M).
+Proof.
+  intro p;unusable_implies_tac 7%nat A p.
+Qed.
+Hint Resolve aux_89 : proof.
+
+Lemma aux_90 : no_proof_for ({P ⊸ M, P, (V ⊸ A) & 1, V}) A.
+Proof.
+  intro p.
+  unusable_var_strong_tac 1%nat 8%nat p.
+Qed.
+Hint Resolve aux_90 : proof.
+
+Lemma aux_91 : no_proof_for ({P ⊸ M, P, (V ⊸ A) & 1, V}) M.
+Proof.
+  intros p; unusable_var_strong_tac 5%nat 6%nat p.
+Qed.
+Hint Resolve aux_91 : proof.
+
+Lemma aux_92 : no_proof_for ({P ⊸ M, P, (V ⊸ A) & 1, V}) (A ⊕ M).
+Proof.
+  intros p; one_step p;eauto with proof.
+(*
+{P ⊸ M, P, (V ⊸ A) & 1, V} ⊢ A e
+{P ⊸ M, P, (V ⊸ A) & 1, V} ⊢ M
+*)
+Qed.
+Hint Resolve aux_92 : proof.
+
+Lemma aux_93 : no_proof_for ({1, P ⊸ M, P, (V ⊸ A) & 1, V}) A.
+Proof.
+  intro p.
+  unusable_var_strong_tac 1%nat 8%nat p.
+Qed.
+Hint Resolve aux_93 : proof.
+
+Lemma aux_94 : no_proof_for ({1, P ⊸ M, P, (V ⊸ A) & 1, V}) M.
+Proof.
+  intros p; unusable_var_strong_tac 5%nat 6%nat p.
+
+Qed.
+Hint Resolve aux_94 : proof.
+
+Lemma aux_77 : no_proof_for ({1, P, (V ⊸ A) & 1, V}) P.
+Proof.
+  intros p; unusable_var_strong_tac 5%nat 6%nat p.
+Qed.
+Hint Resolve aux_77 : proof.
+
+Lemma aux_95 : no_proof_for ({1, P ⊸ M, P, (V ⊸ A) & 1, V}) (A ⊕ M).
+Proof.
+  intros p; one_step p;eauto with proof.
+(*
+{P ⊸ M, P, (V ⊸ A) & 1, V} ⊢ A ⊕ M
+*{1, P ⊸ M, P, (V ⊸ A) & 1, V} ⊢ A e
+{1, P ⊸ M, P, (V ⊸ A) & 1, V} ⊢ M
+{1, P, (V ⊸ A) & 1, V} ⊢ P
+*)
+Qed.
+Hint Resolve aux_95 : proof.
+
+
+Lemma aux_97 : no_proof_for ({P ⊸ M, P, (V ⊸ A) & 1, (E ⊸ A) & 1, V}) A.
+Proof.
+  intro p.
+  unusable_var_strong_tac 1%nat 8%nat p.
+Qed.
+Hint Resolve aux_97 : proof.
+
+
+Lemma aux_99 : no_proof_for ({P ⊸ M, P, (V ⊸ A) & 1, (E ⊸ A) & 1, V}) M.
+Proof.
+  intros p; unusable_var_strong_tac 5%nat 6%nat p.
+Qed.
+Hint Resolve aux_99 : proof.
+
+
+Lemma aux_100 : no_proof_for ({P ⊸ M, P, (V ⊸ A) & 1, (E ⊸ A) & 1, V}) (A ⊕ M).
+Proof.
+  intros p; one_step p;eauto with proof.
+(*
+{P, (V ⊸ A) & 1, (E ⊸ A) & 1, V} ⊢ P
+{P, (V ⊸ A) & 1, V} ⊢ P
+{M, (V ⊸ A) & 1, (E ⊸ A) & 1, V} ⊢ A ⊕ M
+{M, (V ⊸ A) & 1, V} ⊢ A ⊕ M
+{E ⊸ A, P ⊸ M, P, (V ⊸ A) & 1, V} ⊢ A ⊕ M
+{1, P ⊸ M, P, (V ⊸ A) & 1, V} ⊢ A ⊕ M
+{P ⊸ M, P, (V ⊸ A) & 1, (E ⊸ A) & 1, V} ⊢ A e
+{P ⊸ M, P, (V ⊸ A) & 1, (E ⊸ A) & 1, V} ⊢ M e
+*)
+Qed.
+Hint Resolve aux_100 : proof.
+
+Lemma aux_101 : no_proof_for ({P, (V ⊸ A) & 1, (P ⊸ M) & 1, V}) A.
+Proof.
+  intros p; unusable_var_strong_tac 1%nat 8%nat p.
+Qed.
+Hint Resolve aux_101 : proof.
+
+Lemma aux_102 : no_proof_for ({P, (V ⊸ A) & 1, (P ⊸ M) & 1, V}) M.
+Proof.
+  intros p; unusable_var_strong_tac 5%nat 6%nat p.
+Qed.
+Hint Resolve aux_102 : proof.
+
+Lemma aux_103 : no_proof_for ({P, (V ⊸ A) & 1, (P ⊸ M) & 1, V}) (A ⊕ M).
+Proof.
+  intros p; one_step p;eauto with proof.
+(*
+{P, (V ⊸ A) & 1, (P ⊸ M) & 1, V} ⊢ A
+{P, (V ⊸ A) & 1, (P ⊸ M) & 1, V} ⊢ M
+*)
+Qed.
+Hint Resolve aux_103 : proof.
+
+Lemma aux_104 : no_proof_for ({1, P, (V ⊸ A) & 1, (P ⊸ M) & 1, V}) A.
+Proof.
+  intros p; unusable_var_strong_tac 1%nat 8%nat p.
+Qed.
+Hint Resolve aux_104 : proof.
+
+Lemma aux_105 : no_proof_for ({1, P, (V ⊸ A) & 1, (P ⊸ M) & 1, V}) M.
+Proof.
+  intros p; unusable_var_strong_tac 5%nat 6%nat p.
+Qed.
+Hint Resolve aux_105 : proof.
+
+Lemma aux_106 : no_proof_for ({1, P, (V ⊸ A) & 1, (P ⊸ M) & 1, V}) (A ⊕ M).
+Proof.
+  intros p; one_step p;eauto with proof.
+(*
+{P, (V ⊸ A) & 1, (P ⊸ M) & 1, V} ⊢ A ⊕ M
+{1, P, (V ⊸ A) & 1, (P ⊸ M) & 1, V} ⊢ A
+{1, P, (V ⊸ A) & 1, (P ⊸ M) & 1, V} ⊢ M
+*)
+Qed.
+Hint Resolve aux_106 : proof.
+
+Lemma aux_108 : no_proof_for ({P, (V ⊸ A) & 1, (E ⊸ A) & 1, (P ⊸ M) & 1, V}) A.
+Proof.
+  intros p; unusable_var_strong_tac 1%nat 8%nat p.
+Qed.
+Hint Resolve aux_108 : proof.
+
+Lemma aux_110 : no_proof_for ({P, (V ⊸ A) & 1, (E ⊸ A) & 1, (P ⊸ M) & 1, V}) M.
+Proof.
+  intro p;unusable_var_strong_tac 5%nat 6%nat p.
+Qed.
+Hint Resolve aux_110 : proof.
+
+Lemma aux_111 : no_proof_for ({P, (V ⊸ A) & 1, (E ⊸ A) & 1, (P ⊸ M) & 1, V}) (A ⊕ M).
+Proof.
+  intros p; one_step p;eauto with proof.
+(*
+{V ⊸ A, P, (E ⊸ A) & 1, (P ⊸ M) & 1, V} ⊢ A ⊕ M
+{E ⊸ A, P, (V ⊸ A) & 1, (P ⊸ M) & 1, V} ⊢ A ⊕ M
+{P ⊸ M, P, (V ⊸ A) & 1, (E ⊸ A) & 1, V} ⊢ A ⊕ M
+{1, P, (V ⊸ A) & 1, (P ⊸ M) & 1, V} ⊢ A ⊕ M
+{P, (V ⊸ A) & 1, (E ⊸ A) & 1, (P ⊸ M) & 1, V} ⊢ A
+{P, (V ⊸ A) & 1, (E ⊸ A) & 1, (P ⊸ M) & 1, V} ⊢ M
+*)
+Qed.
+Hint Resolve aux_111 : proof.
+
+Lemma aux_200 : no_proof_for ({P ⊸ M, A}) (A ⊕ M).
+Proof.
+  intro p;unusable_implies_tac 1%nat M p.
+Qed.
+Hint Resolve aux_200 : proof.
+
+Lemma aux_201 : all_proofs_of ({A, (P ⊸ M) & 1}) (A ⊕ M).
+Proof.
+  intros p; one_step p;eauto with proof.
+(*
+{P ⊸ M, A} ⊢ A ⊕ M -
+*)
+Qed.
+Hint Resolve aux_201 : proof.
+Hint Rewrite aux_201 : proof.
+
+Lemma aux_202 : no_proof_for ({E ⊸ A, A, (P ⊸ M) & 1}) (A ⊕ M). 
+Proof.
+  intro p;unusable_implies_tac 7%nat A p.
+Qed.
+Hint Resolve aux_202 : proof.
+
+Lemma aux_203 : no_proof_for ({P ⊸ M, A, (E ⊸ A) & 1}) (A ⊕ M).
+Proof.
+  intro p;unusable_implies_tac 1%nat M p.
+Qed.
+Hint Resolve aux_203 : proof.
+
+Lemma aux_204 : no_proof_for ({P ⊸ M, 1, A}) (A ⊕ M).
+Proof.
+  intro p;unusable_implies_tac 1%nat M p.
+Qed.
+Hint Resolve aux_204 : proof.
+
+Lemma aux_205 : all_proofs_of ({1, A, (P ⊸ M) & 1}) (A ⊕ M).
+Proof.
+  intros p; one_step p;eauto with proof.
+(* 
+{P ⊸ M, 1, A} ⊢ A ⊕ M
+ *)
+Qed.
+Hint Resolve aux_205 : proof.
+Hint Rewrite aux_205 : proof.
+
+Lemma aux_206 : no_proof_for ({E ⊸ A, A}) (A ⊕ M).
+Proof.
+  intro p;unusable_implies_tac 7%nat A p.
+Qed.
+Hint Resolve aux_206 : proof.
+
+Lemma aux_207 : all_proofs_of ({A, (E ⊸ A) & 1}) (A ⊕ M).
+Proof.
+  intros p; one_step p;eauto with proof.
+(* 
+   {E ⊸ A, A} ⊢ A ⊕ M
+*)
+Qed.
+Hint Resolve aux_207 : proof.
+Hint Rewrite aux_207 : proof.
+
+Lemma aux_208 : no_proof_for ({E ⊸ A, 1, A}) (A ⊕ M).
+Proof.
+  intro p;unusable_implies_tac 7%nat A p.
+Qed.
+Hint Resolve aux_208 : proof.
+
+Lemma aux_209 : all_proofs_of ({1, A, (E ⊸ A) & 1}) (A ⊕ M).
+Proof.
+  intros p; one_step p;eauto with proof.
+(* 
+   {A, (E ⊸ A) & 1} ⊢ A ⊕ M + 
+   {E ⊸ A, 1, A} ⊢ A ⊕ M - e
+*)
+Qed.
+Hint Resolve aux_209 : proof.
+Hint Rewrite aux_209 : proof.
+
+Lemma aux_210 : all_proofs_of ({A, (E ⊸ A) & 1, (P ⊸ M) & 1}) (A ⊕ M).
+Proof.
+  intros p; one_step p;eauto with proof.
+(*
+{E ⊸ A, A, (P ⊸ M) & 1} ⊢ A ⊕ M - e
+{P ⊸ M, A, (E ⊸ A) & 1} ⊢ A ⊕ M - e
+{1, A, (P ⊸ M) & 1} ⊢ A ⊕ M  + 
+{1, A, (E ⊸ A) & 1} ⊢ A ⊕ M  +
+*)
+Qed.
+Hint Resolve aux_210 : proof.
+Hint Rewrite aux_210 : proof.
+
+Lemma aux_211 : no_proof_for ({E ⊸ A, A, P & 1, (P ⊸ M) & 1}) (A ⊕ M).
+Proof.
+  intro p;unusable_implies_tac 7%nat A p.
+Qed.
+Hint Resolve aux_211 : proof.
+
+Lemma aux_212 : no_proof_for ({E ⊸ A, P ⊸ M, A, P & 1}) (A ⊕ M).
+Proof.
+  intro p;unusable_implies_tac 7%nat A p.
+Qed.
+Hint Resolve aux_212 : proof.
+
+Lemma aux_213 : no_proof_for ({1, P ⊸ M, A, (E ⊸ A) & 1}) (A ⊕ M).
+Proof.
+  intro p;unusable_implies_tac 1%nat M p.
+Qed.
+Hint Resolve aux_213 : proof.
+
+Lemma aux_214 : no_proof_for ({1, P ⊸ M, A}) A.
+Proof.
+  intro p;unusable_implies_tac 1%nat M p.
+Qed.
+Hint Resolve aux_214 : proof.
+
+Lemma aux_215 : no_proof_for ({P ⊸ M, A, P & 1}) (A).
+Proof.
+  intros p; one_step p;eauto with proof.
+(*
+{1, P ⊸ M, A} ⊢ A
+*)
+Qed. 
+Hint Resolve aux_215 : proof.
+
+Lemma aux_216 : no_proof_for ({P ⊸ M, A, P & 1}) (A ⊕ M).
+Proof.
+  intros p; one_step p;eauto with proof.
+(*
+{P ⊸ M, A, P & 1} ⊢ A
+*)
+Qed.
+Hint Resolve aux_216 : proof.
+
+Lemma aux_217 : no_proof_for ({1, 1, P ⊸ M, A}) (A ⊕ M).
+Proof.
+  intro p;unusable_implies_tac 1%nat M p.
+Qed.
+Hint Resolve aux_217 : proof.
+
+Lemma aux_218 : no_proof_for ({1, 1, P ⊸ M, A}) A.
+Proof.
+  intro p;unusable_implies_tac 1%nat M p.
+Qed.
+Hint Resolve aux_218 : proof.
+
+Lemma aux_219 : no_proof_for ({1, P ⊸ M, A, P & 1}) A.
+Proof.
+  intros p; one_step p;eauto with proof.
+(*
+{1, 1, P ⊸ M, A} ⊢ A
+*)
+Qed.
+Hint Resolve aux_219 : proof.
+
+Lemma aux_220 : no_proof_for ({1, P ⊸ M, A, P & 1}) (A ⊕ M).
+Proof.
+  intros p; one_step p;eauto with proof.
+(*
+{P ⊸ M, A, P & 1} ⊢ A ⊕ M
+{1, 1, P ⊸ M, A} ⊢ A ⊕ M e
+{1, P ⊸ M, A, P & 1} ⊢ A
+*)
+Qed.
+Hint Resolve aux_220 : proof.
+
+
+Lemma aux_221 : all_proofs_of ({P ⊸ M, A, P & 1, (E ⊸ A) & 1}) (A ⊕ M).
+Proof.
+  intros p; one_step p;eauto with proof.
+(*
+{E ⊸ A, P ⊸ M, A, P & 1} ⊢ A ⊕ M  - e 
+{1, P ⊸ M, A, (E ⊸ A) & 1} ⊢ A ⊕ M - e
+{1, P ⊸ M, A, P & 1} ⊢ A ⊕ M - 
+*)
+Qed.
+Hint Resolve aux_221 : proof.
+Hint Rewrite aux_221 : proof.
+
+Lemma aux_222 : no_proof_for ({E ⊸ A, 1, A, (P ⊸ M) & 1}) (A ⊕ M).
+Proof.
+  intro p;unusable_implies_tac 7%nat A p.
+Qed.
+Hint Resolve aux_222 : proof.
+
+Lemma aux_223 : all_proofs_of ({1, 1, A, (P ⊸ M) & 1}) (A ⊕ M).
+Proof.
+  intros p; one_step p;eauto with proof.
+Qed.
+Hint Resolve aux_223 : proof.
+Hint Rewrite aux_223 : proof.
+
+
+Lemma aux_224 : no_proof_for ({E ⊸ A, 1, 1, A}) (A ⊕ M).
+Proof.
+  intro p;unusable_implies_tac 7%nat A p.
+Qed.
+Hint Resolve aux_224 : proof.
+
+Lemma aux_225 : all_proofs_of ({1, 1, A, (E ⊸ A) & 1}) (A ⊕ M).
+Proof.
+  intros p; one_step p;eauto with proof.
+(*
+{E ⊸ A, 1, 1, A} ⊢ A ⊕ M
+*)
+Qed.
+Hint Resolve aux_225 : proof.
+Hint Rewrite aux_225 : proof.
+
+Lemma aux_226 : all_proofs_of ({1, A, (E ⊸ A) & 1, (P ⊸ M) & 1}) (A ⊕ M).
+Proof.
+  intros p; one_step p;eauto with proof.
+(*
+{E ⊸ A, 1, A, (P ⊸ M) & 1} ⊢ A ⊕ M - e
+{1, 1, A, (P ⊸ M) & 1} ⊢ A ⊕ M     +
+{1, 1, A, (E ⊸ A) & 1} ⊢ A ⊕ M     +
+*)
+Qed.
+Hint Resolve aux_226 : proof.
+Hint Rewrite aux_226 : proof.
+
+Lemma aux_227 : all_proofs_of ({A, P & 1}) (A ⊕ M).
+Proof.
+  intros p; one_step p;eauto with proof.
+Qed.
+Hint Resolve aux_227 : proof.
+Hint Rewrite aux_227 : proof.
+
+Lemma aux_228 : all_proofs_of ({1, A, P & 1}) (A ⊕ M).
+Proof.
+  intros p; one_step p;eauto with proof.
+(*
+   {A, P & 1} ⊢ (A ⊕ M)
+*)
+Qed.
+Hint Resolve aux_228 : proof.
+Hint Rewrite aux_228 : proof.
+
+
+Lemma aux_229 : all_proofs_of ({A, P & 1, (P ⊸ M) & 1}) (A ⊕ M).
+Proof.
+  intros p; one_step p;eauto with proof.
+(*
+   {1, A, P & 1} ⊢ A ⊕ M +
+*)
+Qed.
+Hint Resolve aux_229 : proof.
+Hint Rewrite aux_229 : proof.
+
+Lemma aux_230 : all_proofs_of ({1, 1, A, P & 1}) (A ⊕ M).
+Proof.
+  intros p; one_step p;eauto with proof.
+Qed.
+Hint Resolve aux_230 : proof.
+Hint Rewrite aux_230 : proof.
+
+
+Lemma aux_231 : all_proofs_of ({1, A, P & 1, (P ⊸ M) & 1}) (A ⊕ M).
+Proof.
+  intros p; one_step p;eauto with proof.
+(*
+{A, P & 1, (P ⊸ M) & 1} ⊢ A ⊕ M + 
+{1, 1, A, P & 1} ⊢ A ⊕ M +
+*)
+Qed.
+Hint Resolve aux_231 : proof.
+Hint Rewrite aux_231 : proof.
+
+Lemma aux_232 : no_proof_for ({E ⊸ A, A, P & 1}) (A ⊕ M).
+Proof.
+  intro p;unusable_implies_tac 7%nat A p.
+Qed.
+Hint Resolve aux_232 : proof.
+
+Lemma aux_233 : all_proofs_of ({A, P & 1, (E ⊸ A) & 1}) (A ⊕ M).
+Proof.
+  intros p; one_step p;eauto with proof.
+(*
+{E ⊸ A, A, P & 1} ⊢ A ⊕ M - e
+*)
+Qed.
+Hint Resolve aux_233 : proof.
+Hint Rewrite aux_233 : proof.
+
+Lemma aux_234 : no_proof_for ({E ⊸ A, 1, A, P & 1}) (A ⊕ M).
+Proof.
+  intro p;unusable_implies_tac 7%nat A p.
+Qed.
+Hint Resolve aux_234 : proof.
+
+Lemma aux_235 : all_proofs_of ({1, A, P & 1, (E ⊸ A) & 1}) (A ⊕ M).
+Proof.
+  intros p; one_step p;eauto with proof.
+(*
+ {A, P & 1, (E ⊸ A) & 1} ⊢ A ⊕ M + 
+ {E ⊸ A, 1, A, P & 1} ⊢ A ⊕ M - e
+*)
+Qed.
+Hint Resolve aux_235 : proof.
+Hint Rewrite aux_235 : proof.
+
+Lemma aux_236 : all_proofs_of ({A, P & 1, (E ⊸ A) & 1, (P ⊸ M) & 1}) (A ⊕ M).
+Proof.
+  intros p; one_step p;eauto with proof.
+(* 
+{E ⊸ A, A, P & 1, (P ⊸ M) & 1} ⊢ A ⊕ M       - e
+{P ⊸ M, A, P & 1, (E ⊸ A) & 1} ⊢ A ⊕ M       + 
+{1, A, (E ⊸ A) & 1, (P ⊸ M) & 1} ⊢ A ⊕ M     +
+{1, A, P & 1, (P ⊸ M) & 1} ⊢ A ⊕ M           +
+*)
+Qed.
+Hint Resolve aux_236 : proof.
+Hint Rewrite aux_236 : proof.
+
+Lemma aux_237 : no_proof_for ({E ⊸ A, V ⊸ A, P & 1, (P ⊸ M) & 1, V}) (A ⊕ M).
+Proof.
+  intro p;unusable_implies_tac 7%nat A p.
+Qed.
+Hint Resolve aux_237 : proof.
+
+Lemma aux_238 : no_proof_for ({V ⊸ A, P & 1, (E ⊸ A) & 1, V}) P.
+Proof.
+  intro p; unusable_var_strong_tac 5%nat 6%nat p.
+Qed.
+Hint Resolve aux_238 : proof.
+
+Lemma aux_239 : no_proof_for ({V ⊸ A, P & 1, V}) P.
+Proof.
+  intro p; unusable_var_strong_tac 5%nat 6%nat p.
+Qed.
+Hint Resolve aux_239 : proof.
+
+Lemma aux_240 : no_proof_for ({E ⊸ A, P ⊸ M, P & 1, V}) V.
+Proof.
+  intro p;unusable_implies_tac 7%nat A p.
+Qed.
+Hint Resolve aux_240 : proof.
+
+Lemma aux_241 : no_proof_for ({1, P ⊸ M, (E ⊸ A) & 1, V}) V.
+Proof.
+  intro p;unusable_implies_tac 1%nat M p.
+Qed.
+Hint Resolve aux_241 : proof.
+
+Lemma aux_242 : no_proof_for ({1, P ⊸ M, V}) V.
+Proof.
+  intro p;unusable_implies_tac 1%nat M p.
+Qed.
+Hint Resolve aux_242 : proof.
+
+Lemma aux_243 : no_proof_for ({P ⊸ M, P & 1, V}) V.
+Proof.
+  intro p;one_step p;eauto with proof.
+(*
+   {1, P ⊸ M, V} ⊢ V e
+*)
+Qed.
+Hint Resolve aux_243 : proof.
+
+Lemma aux_244 : no_proof_for ({1, 1, P ⊸ M, V}) V.
+Proof.
+  intro p;unusable_implies_tac 1%nat M p.
+Qed.
+Hint Resolve aux_244 : proof.
+
+Lemma aux_245 : no_proof_for ({1, P ⊸ M, P & 1, V}) V.
+Proof.
+  intro p;one_step p;eauto with proof.
+(*
+{P ⊸ M, P & 1, V} ⊢ V        
+{1, 1, P ⊸ M, V} ⊢ V         e 
+*)
+Qed.
+Hint Resolve aux_245 : proof.
+
+Lemma aux_246 : no_proof_for ({P ⊸ M, P & 1, (E ⊸ A) & 1, V}) V.
+Proof.
+  intros p; one_step p;eauto with proof.
+(* 
+{E ⊸ A, P ⊸ M, P & 1, V} ⊢ V     e
+{1, P ⊸ M, (E ⊸ A) & 1, V} ⊢ V   e
+{1, P ⊸ M, P & 1, V} ⊢ V          
+*)
+Qed.
+Hint Resolve aux_246 : proof.
+Hint Rewrite aux_246 : proof.
+
+Lemma aux_247 : no_proof_for ({P ⊸ M, V}) V.
+Proof.
+  intro p;unusable_implies_tac 1%nat M p.
+Qed.
+Hint Resolve aux_247 : proof.
+
+Lemma aux_248 : no_proof_for ({P ⊸ M, (E ⊸ A) & 1, V}) V.
+Proof.
+  intro p;unusable_implies_tac 1%nat M p.
+Qed.
+Hint Resolve aux_248 : proof.
+
+Lemma aux_249 : no_proof_for ({E ⊸ A, A, P ⊸ M, P & 1}) A.
+Proof.
+  intro p;unusable_implies_tac 7%nat A p.
+Qed.
+Hint Resolve aux_249 : proof.
+
+Lemma aux_250 : no_proof_for ({1, A, P ⊸ M, (E ⊸ A) & 1}) A.
+Proof.
+  intro p;unusable_implies_tac 1%nat M p.
+Qed.
+Hint Resolve aux_250 : proof.
+
+Lemma aux_251 : no_proof_for ({A, P ⊸ M, P & 1, (E ⊸ A) & 1}) A.
+Proof.
+  intros p; one_step p;eauto with proof.
+(*
+ {E ⊸ A, A, P ⊸ M, P & 1} ⊢ A   e
+{1, A, P ⊸ M, (E ⊸ A) & 1} ⊢ A   e
+*)
+Qed.
+Hint Resolve aux_251 : proof.
+
+Lemma aux_252 : no_proof_for ({A, P ⊸ M, P & 1, (E ⊸ A) & 1}) (A ⊕ M).
+Proof.
+  intros p; one_step p;eauto with proof.
+(*
+ {A, P ⊸ M, P & 1, (E ⊸ A) & 1} ⊢ A
+*)
+Qed.
+Hint Resolve aux_252 : proof.
+
+Lemma aux_253 : no_proof_for ({E ⊸ A, P ⊸ M, V ⊸ A, P & 1, V}) (A ⊕ M).
+Proof.
+  intro p;unusable_implies_tac 7%nat A p.
+Qed.
+Hint Resolve aux_253 : proof.
+
+Lemma aux_254 : no_proof_for ({E ⊸ A, P ⊸ M, V ⊸ A, V}) (A ⊕ M).
+Proof.
+  intro p;unusable_implies_tac 7%nat A p.
+Qed.
+Hint Resolve aux_254 : proof.
+
+Lemma aux_255 : no_proof_for ({P ⊸ M, V ⊸ A, V}) A.
+Proof.
+  intro p;unusable_implies_tac 1%nat M p.
+Qed.
+Hint Resolve aux_255 : proof.
+
+Lemma aux_256 : no_proof_for ({P ⊸ M, V ⊸ A, V}) M.
+Proof.
+  intro p;unusable_var_strong_tac 5%nat 6%nat p.
+Qed.
+Hint Resolve aux_256 : proof.
+
+Lemma aux_257 : no_proof_for ({P ⊸ M, V ⊸ A, V}) (A ⊕ M).
+Proof.
+  intros p; one_step p;eauto with proof.
+(*
+{P ⊸ M, V ⊸ A, V} ⊢ A e
+{P ⊸ M, V ⊸ A, V} ⊢ M e
+*)
+Qed.
+Hint Resolve aux_257 : proof.
+
+Lemma aux_258 : no_proof_for ({1, P ⊸ M, V ⊸ A, V}) A.
+Proof.
+  intro p;unusable_implies_tac 1%nat M p.
+Qed.
+Hint Resolve aux_258 : proof.
+
+Lemma aux_259 : no_proof_for ({1, P ⊸ M, V ⊸ A, V}) M.
+Proof.
+  intro p;unusable_var_strong_tac 5%nat 6%nat p.
+Qed.
+Hint Resolve aux_259 : proof.
+
+Lemma aux_260 : no_proof_for ({1, P ⊸ M, V ⊸ A, V}) (A ⊕ M).
+Proof.
+  intros p; one_step p;eauto with proof.
+(*
+{P ⊸ M, V ⊸ A, V} ⊢ A ⊕ M
+{1, P ⊸ M, V ⊸ A, V} ⊢ A      e
+{1, P ⊸ M, V ⊸ A, V} ⊢ M      e
+*)
+Qed.
+Hint Resolve aux_260 : proof.
+
+Lemma aux_261 : no_proof_for ({P ⊸ M, V ⊸ A, (E ⊸ A) & 1, V}) A.
+Proof.
+  intro p;unusable_implies_tac 1%nat M p.
+Qed.
+Hint Resolve aux_261 : proof.
+
+Lemma aux_262 : no_proof_for ({P ⊸ M, V ⊸ A, (E ⊸ A) & 1, V}) M.
+Proof.
+  intro p;unusable_var_strong_tac 5%nat 6%nat p.
+Qed.
+Hint Resolve aux_262 : proof.
+
+Lemma aux_263 : no_proof_for ({P ⊸ M, V ⊸ A, (E ⊸ A) & 1, V}) (A ⊕ M).
+Proof.
+  intros p; one_step p;eauto with proof.
+(*
+{E ⊸ A, P ⊸ M, V ⊸ A, V} ⊢ A ⊕ M  e
+{1, P ⊸ M, V ⊸ A, V} ⊢ A ⊕ M 
+{P ⊸ M, V ⊸ A, (E ⊸ A) & 1, V} ⊢ A  e
+{P ⊸ M, V ⊸ A, (E ⊸ A) & 1, V} ⊢ M  e
+*)
+Qed.
+Hint Resolve aux_263 : proof.
+
+Lemma aux_264 : no_proof_for ({E ⊸ A, 1, P ⊸ M, V ⊸ A, V}) (A ⊕ M).
+Proof.
+  intro p;unusable_implies_tac 7%nat A p.
+Qed.
+Hint Resolve aux_264 : proof.
+
+
+Lemma aux_265 : no_proof_for ({1, 1, P ⊸ M, V ⊸ A, V}) A.
+Proof.
+  intro p;unusable_implies_tac 1%nat M p.
+Qed.
+Hint Resolve aux_265 : proof.
+
+Lemma aux_266 : no_proof_for ({1, 1, P ⊸ M, V ⊸ A, V}) M.
+Proof.
+  intro p;unusable_var_strong_tac 5%nat 6%nat p.
+Qed.
+Hint Resolve aux_266 : proof.
+
+Lemma aux_267 : no_proof_for ({1, 1, P ⊸ M, V ⊸ A, V}) (A ⊕ M).
+Proof.
+  intros p; one_step p;eauto with proof.
+(*
+{1, 1, P ⊸ M, V ⊸ A, V} ⊢ A  e
+{1, 1, P ⊸ M, V ⊸ A, V} ⊢ M  e
+*)
+Qed.
+Hint Resolve aux_267 : proof.
+
+Lemma aux_268 : no_proof_for ({1, P ⊸ M, V ⊸ A, (E ⊸ A) & 1, V}) A.
+Proof.
+  intro p;unusable_implies_tac 1%nat M p.
+Qed.
+Hint Resolve aux_268 : proof.
+
+Lemma aux_269 : no_proof_for ({1, P ⊸ M, V ⊸ A, (E ⊸ A) & 1, V}) M.
+Proof.
+  intro p;unusable_var_strong_tac 5%nat 6%nat p.
+Qed.
+Hint Resolve aux_269 : proof.
+
+Lemma aux_270 : no_proof_for ({1, P ⊸ M, V ⊸ A, (E ⊸ A) & 1, V}) (A ⊕ M).
+Proof.
+  intros p; one_step p;eauto with proof.
+(*
+{P ⊸ M, V ⊸ A, (E ⊸ A) & 1, V} ⊢ A ⊕ M
+{E ⊸ A, 1, P ⊸ M, V ⊸ A, V} ⊢ A ⊕ M        e
+{1, 1, P ⊸ M, V ⊸ A, V} ⊢ A ⊕ M
+{1, P ⊸ M, V ⊸ A, (E ⊸ A) & 1, V} ⊢ A      e
+{1, P ⊸ M, V ⊸ A, (E ⊸ A) & 1, V} ⊢ M      e
+*)
+Qed.
+Hint Resolve aux_270 : proof.
+
+Lemma aux_301 : no_proof_for ({1, V ⊸ A, P & 1, V}) P.
+Proof.
+  intro p;unusable_var_strong_tac 5%nat 6%nat p.
+Qed.
+Hint Resolve aux_301 : proof.
+
+Lemma aux_302 : no_proof_for ({A, P ⊸ M}) A.
+Proof.
+  intro p. unusable_implies_tac 1%nat M p.
+Qed.
+Hint Resolve aux_302 : proof.
+
+Lemma aux_303 : no_proof_for ({P ⊸ M, V ⊸ A, P & 1, V}) A.
+Proof.
+  intros p; one_step p;eauto with proof.
+(*
+   {A, P ⊸ M} ⊢ A e
+*)
+Qed.
+Hint Resolve aux_303 : proof.
+
+Lemma aux_304 : no_proof_for ({P ⊸ M, V ⊸ A, P & 1, V}) M.
+Proof.
+  intro p;unusable_var_strong_tac 5%nat 6%nat p.
+Qed.
+Hint Resolve aux_304 : proof.
+
+Lemma aux_305 : no_proof_for ({P ⊸ M, V ⊸ A, P & 1, V}) (A ⊕ M).
+Proof.
+  intros p; one_step p;eauto with proof.
+(*
+{P ⊸ M, V ⊸ A, P & 1, V} ⊢ A    
+{P ⊸ M, V ⊸ A, P & 1, V} ⊢ M    e
+*)
+Qed.
+Hint Resolve aux_305 : proof.
+
+Lemma aux_306 : no_proof_for ({1, P ⊸ M, V ⊸ A, P & 1, V}) A.
+Proof.
+  intros p; one_step p;eauto with proof.
+Qed.
+Hint Resolve aux_306 : proof.
+
+Lemma aux_307 : no_proof_for ({1, P ⊸ M, V ⊸ A, P & 1, V}) M.
+Proof.
+  intros p; unusable_var_strong_tac 5%nat 6%nat p.
+Qed.
+Hint Resolve aux_307 : proof.
+
+Lemma aux_308 : no_proof_for ({1, P ⊸ M, V ⊸ A, P & 1, V}) (A ⊕ M).
+Proof.
+  intros p; one_step p;eauto with proof.
+(*
+{1, V ⊸ A, P & 1, V} ⊢ P   e
+{P ⊸ M, V ⊸ A, P & 1, V} ⊢ A ⊕ M
+{1, P ⊸ M, V ⊸ A, P & 1, V} ⊢ A 
+{1, P ⊸ M, V ⊸ A, P & 1, V} ⊢ M  e
+*)
+Qed.
+Hint Resolve aux_308 : proof.
+
+Lemma aux_310 : no_proof_for ({A, P ⊸ M, (E ⊸ A) & 1}) A.
+Proof.
+  intro p. unusable_implies_tac 1%nat M p.
+Qed.
+Hint Resolve aux_310 : proof.
+
+Lemma aux_311 : no_proof_for ({E ⊸ A, P ⊸ M, V ⊸ A, P & 1, V}) A.
+Proof.
+  intro p. unusable_implies_tac 7%nat A p.
+Qed.
+Hint Resolve aux_311 : proof.
+
+Lemma aux_309 : no_proof_for ({P ⊸ M, V ⊸ A, P & 1, (E ⊸ A) & 1, V}) A.
+Proof.
+  intros p; one_step p;eauto with proof.
+(*
+{A, P ⊸ M, (E ⊸ A) & 1} ⊢ A e 
+{E ⊸ A, P ⊸ M, V ⊸ A, P & 1, V} ⊢ A e
+*)
+Qed.
+Hint Resolve aux_309 : proof.
+
+Lemma aux_312 : no_proof_for ({P ⊸ M, V ⊸ A, P & 1, (E ⊸ A) & 1, V}) M.
+Proof.
+  intros p; unusable_var_strong_tac 5%nat 6%nat p.
+Qed.
+Hint Resolve aux_312 : proof.
+     
+Lemma aux_300 : no_proof_for ({P ⊸ M, V ⊸ A, P & 1, (E ⊸ A) & 1, V}) (A ⊕ M).
+Proof.
+  intros p; one_step p;eauto with proof.
+(*
+{V ⊸ A, P & 1, (E ⊸ A) & 1, V} ⊢ P              e
+{V ⊸ A, P & 1, V} ⊢ P                           e 
+{P ⊸ M, P & 1, (E ⊸ A) & 1, V} ⊢ V
+{P ⊸ M, P & 1, V} ⊢ V
+{P ⊸ M, V} ⊢ V                                  e
+{P ⊸ M, (E ⊸ A) & 1, V} ⊢ V                     e
+{A, P ⊸ M, P & 1, (E ⊸ A) & 1} ⊢ A ⊕ M
+{E ⊸ A, P ⊸ M, V ⊸ A, P & 1, V} ⊢ A ⊕ M        e
+{1, P ⊸ M, V ⊸ A, (E ⊸ A) & 1, V} ⊢ A ⊕ M
+{1, P ⊸ M, V ⊸ A, P & 1, V} ⊢ A ⊕ M
+{P ⊸ M, V ⊸ A, P & 1, (E ⊸ A) & 1, V} ⊢ A      
+{P ⊸ M, V ⊸ A, P & 1, (E ⊸ A) & 1, V} ⊢ M      e
+*)
+Qed.
+Hint Resolve aux_300 : proof.
+
+Lemma aux_313 : all_proofs_of ({A, 1, (E ⊸ A) & 1, (P ⊸ M) & 1}) (A ⊕ M).
+Proof.
+  intros p; eauto 2 with proof.
+Qed.
+Hint Resolve aux_313 : proof.
+Hint Rewrite aux_313 : proof.
+
+Lemma aux_314 : all_proofs_of ({A, 1, (E ⊸ A) & 1}) (A ⊕ M).
+Proof.
+  intros p; one_step p;eauto with proof. 
+Qed.
+Hint Resolve aux_314 : proof.
+Hint Rewrite aux_314 : proof.
+
+Lemma aux_315 : all_proofs_of ({A, 1, (P ⊸ M) & 1}) (A ⊕ M).
+Proof.
+  intros p; one_step p;eauto with proof. 
+Qed.
+Hint Resolve aux_315 : proof.
+Hint Rewrite aux_315 : proof.
+
+Lemma aux_316 : no_proof_for ({E ⊸ A, V ⊸ A, (P ⊸ M) & 1, V}) (A ⊕ M).
+Proof.
+  intros p; unusable_implies_tac 7%nat A p.
+Qed.
+Hint Resolve aux_316 : proof.
+
+Lemma aux_317 : no_proof_for ({V ⊸ A, (P ⊸ M) & 1, V}) M.
+Proof.
+  intros p; unusable_var_strong_tac 5%nat 6%nat p.
+Qed.
+Hint Resolve aux_317 : proof.
+
+Lemma aux_318 : all_proofs_of ({V ⊸ A, (P ⊸ M) & 1, V}) (A ⊕ M).
+Proof.
+  intros p; one_step p;eauto with proof. 
+(*
+{V ⊸ A, (P ⊸ M) & 1, V} ⊢ M
+*)
+Qed.
+Hint Resolve aux_318 : proof.
+Hint Rewrite aux_318 : proof.
+
+Lemma aux_319 : no_proof_for ({1, V ⊸ A, (P ⊸ M) & 1, V}) M.
+Proof.
+  intros p; unusable_var_strong_tac 5%nat 6%nat p.
+Qed.
+Hint Resolve aux_319 : proof.
+
+Lemma aux_320 : all_proofs_of ({1, V ⊸ A, (P ⊸ M) & 1, V}) (A ⊕ M).
+Proof.
+  intros p; one_step p;eauto with proof. 
+(*
+{V ⊸ A, (P ⊸ M) & 1, V} ⊢ A ⊕ M        +
+{1, V ⊸ A, (P ⊸ M) & 1, V} ⊢ M         - e
+*)
+Qed.
+Hint Resolve aux_320 : proof.
+Hint Rewrite aux_320 : proof.
+
+Lemma aux_321 : no_proof_for ({E ⊸ A, V ⊸ A, V}) (A ⊕ M).
+Proof.
+  intros p; unusable_implies_tac 7%nat A p.
+Qed.
+Hint Resolve aux_321 : proof.
+
+
+Lemma aux_322 : all_proofs_of ({V ⊸ A, (E ⊸ A) & 1, V}) (A ⊕ M).
+Proof.
+  intros p; one_step p;eauto with proof. 
+(*
+{E ⊸ A, V ⊸ A, V} ⊢ A ⊕ M  e
+*)
+Qed.
+Hint Resolve aux_322 : proof.
+Hint Rewrite aux_322 : proof.
+
+Lemma aux_323 : no_proof_for ({E ⊸ A, 1, V ⊸ A, V}) (A ⊕ M).
+Proof.
+  intros p; unusable_implies_tac 7%nat A p.
+Qed.
+Hint Resolve aux_323 : proof.
+
+Lemma aux_324 : all_proofs_of ({1, V ⊸ A, (E ⊸ A) & 1, V}) (A ⊕ M).
+Proof.
+  intros p; one_step p;eauto with proof. 
+(*
+{V ⊸ A, (E ⊸ A) & 1, V} ⊢ A ⊕ M       +
+{E ⊸ A, 1, V ⊸ A, V} ⊢ A ⊕ M          - e
+*)
+Qed.
+Hint Resolve aux_324 : proof.
+Hint Rewrite aux_324 : proof.
+
+Lemma aux_325 : no_proof_for ({V ⊸ A, (E ⊸ A) & 1, (P ⊸ M) & 1, V}) M.
+Proof.
+  intros p; unusable_var_strong_tac 5%nat 6%nat p.
+Qed.
+Hint Resolve aux_325 : proof.
+
+Lemma aux_326 : all_proofs_of ({V ⊸ A, (E ⊸ A) & 1, (P ⊸ M) & 1, V}) (A ⊕ M).
+Proof.
+  intros p; one_step p;eauto with proof. 
+(*
+{E ⊸ A, V ⊸ A, (P ⊸ M) & 1, V} ⊢ A ⊕ M     - e
+{1, V ⊸ A, (P ⊸ M) & 1, V} ⊢ A ⊕ M         +
+{1, V ⊸ A, (E ⊸ A) & 1, V} ⊢ A ⊕ M         +
+{V ⊸ A, (E ⊸ A) & 1, (P ⊸ M) & 1, V} ⊢ M  - e 
+*)
+Qed.
+Hint Resolve aux_326 : proof.
+Hint Rewrite aux_326 : proof.
+
+Lemma aux_327 : no_proof_for ({E ⊸ A, 1, V ⊸ A, (P ⊸ M) & 1, V}) (A ⊕ M).
+Proof.
+  intros p; unusable_implies_tac 7%nat A p.
+Qed.
+Hint Resolve aux_327 : proof.
+
+
+Lemma aux_328 : all_proofs_of ({A, 1, 1, (P ⊸ M) & 1}) (A ⊕ M).
+Proof.
+  intros p; one_step p;eauto with proof. 
+Qed.
+Hint Resolve aux_328 : proof.
+Hint Rewrite aux_328 : proof.
+
+Lemma aux_329 : no_proof_for ({1, 1, V ⊸ A, (P ⊸ M) & 1, V}) M.
+Proof.
+  intros p; unusable_var_strong_tac 5%nat 6%nat p.
+Qed.
+Hint Resolve aux_329 : proof.
+
+Lemma aux_330 : all_proofs_of ({1, 1, V ⊸ A, (P ⊸ M) & 1, V}) (A ⊕ M).
+Proof.
+  intros p; one_step p;eauto with proof. 
+(*
+{A, 1, 1, (P ⊸ M) & 1} ⊢ A ⊕ M       +
+{1, 1, V ⊸ A, (P ⊸ M) & 1, V} ⊢ M   e - 
+*)
+Qed.
+Hint Resolve aux_330 : proof.
+Hint Rewrite aux_330 : proof.
+
+Lemma aux_331 : all_proofs_of ({A, 1, 1, (E ⊸ A) & 1}) (A ⊕ M).
+Proof.
+  intros p; one_step p;eauto with proof. 
+Qed.
+Hint Resolve aux_331 : proof.
+Hint Rewrite aux_331 : proof.
+
+Lemma aux_332 : no_proof_for ({E ⊸ A, 1, 1, V ⊸ A, V}) (A ⊕ M).
+Proof.
+  intros p; unusable_implies_tac 7%nat A p.
+Qed.
+Hint Resolve aux_332 : proof.
+
+Lemma aux_333 : all_proofs_of ({1, 1, V ⊸ A, (E ⊸ A) & 1, V}) (A ⊕ M).
+Proof.
+  intros p; one_step p;eauto with proof. 
+(*
+{A, 1, 1, (E ⊸ A) & 1} ⊢ A ⊕ M       +
+{E ⊸ A, 1, 1, V ⊸ A, V} ⊢ A ⊕ M     - e
+*)
+Qed.
+Hint Resolve aux_333 : proof.
+Hint Rewrite aux_333 : proof.
+
+Lemma aux_334 : no_proof_for ({1, V ⊸ A, (E ⊸ A) & 1, (P ⊸ M) & 1, V}) M.
+Proof.
+  intros p; unusable_var_strong_tac 5%nat 6%nat p.
+Qed.
+Hint Resolve aux_334 : proof.
+
+Lemma aux_335 : all_proofs_of ({1, V ⊸ A, (E ⊸ A) & 1, (P ⊸ M) & 1, V}) (A ⊕ M).
+Proof.
+  intros p; one_step p;eauto with proof. 
+(*
+{A, 1, (E ⊸ A) & 1, (P ⊸ M) & 1} ⊢ A ⊕ M        +
+{A, 1, (E ⊸ A) & 1} ⊢ A ⊕ M                     +
+{A, 1, (P ⊸ M) & 1} ⊢ A ⊕ M                     +
+{V ⊸ A, (E ⊸ A) & 1, (P ⊸ M) & 1, V} ⊢ A ⊕ M   +
+{E ⊸ A, 1, V ⊸ A, (P ⊸ M) & 1, V} ⊢ A ⊕ M      - e
+{1, 1, V ⊸ A, (P ⊸ M) & 1, V} ⊢ A ⊕ M          +
+{1, 1, V ⊸ A, (E ⊸ A) & 1, V} ⊢ A ⊕ M          + 
+{1, V ⊸ A, (E ⊸ A) & 1, (P ⊸ M) & 1, V} ⊢ M   - e
+*)
+Qed.
+Hint Resolve aux_335 : proof.
+Hint Rewrite aux_335 : proof.
+
+Lemma aux_336 : all_proofs_of ({A, 1, P & 1, (P ⊸ M) & 1}) (A ⊕ M).
+Proof.
+  intros p; one_step p;eauto with proof. 
+Qed.
+Hint Resolve aux_336 : proof.
+Hint Rewrite aux_336 : proof.
+
+Lemma aux_337 : all_proofs_of ({A, 1, P & 1}) (A ⊕ M).
+Proof.
+  intros p; one_step p;eauto with proof. 
+Qed.
+Hint Resolve aux_337 : proof.
+Hint Rewrite aux_337 : proof.
+
+Lemma aux_338 : all_proofs_of ({V ⊸ A, P & 1, V}) (A ⊕ M).
+Proof.
+  intros p; one_step p;eauto with proof. 
+Qed.
+Hint Resolve aux_338 : proof.
+Hint Rewrite aux_338 : proof.
+
+Lemma aux_339 : all_proofs_of ({1, V ⊸ A, P & 1, V}) (A ⊕ M).
+Proof.
+  intros p; one_step p;eauto with proof. 
+(*
+*{V ⊸ A, P & 1, V} ⊢ A ⊕ M
+*)
+Qed.
+Hint Resolve aux_339 : proof.
+Hint Rewrite aux_339 : proof.
+
+Lemma aux_340 : no_proof_for ({V ⊸ A, P & 1, (P ⊸ M) & 1, V}) M.
+Proof.
+  intros p; unusable_var_strong_tac 5%nat 6%nat p.
+Qed.
+Hint Resolve aux_340 : proof.
+
+Lemma aux_341 : all_proofs_of ({V ⊸ A, P & 1, (P ⊸ M) & 1, V}) (A ⊕ M).
+Proof.
+  intros p; one_step p;eauto with proof. 
+(*
+{1, V ⊸ A, P & 1, V} ⊢ A ⊕ M
+{V ⊸ A, P & 1, (P ⊸ M) & 1, V} ⊢ M     - e
+*)
+Qed.
+Hint Resolve aux_341 : proof.
+Hint Rewrite aux_341 : proof.
+
+
+Lemma aux_343 : all_proofs_of ({A, 1, 1, P & 1}) (A ⊕ M).
+Proof.
+  intros p; one_step p;eauto with proof. 
+Qed.
+Hint Resolve aux_343 : proof.
+Hint Rewrite aux_343 : proof.
+
+Lemma aux_342 : all_proofs_of ({1, 1, V ⊸ A, P & 1, V}) (A ⊕ M).
+Proof.
+  intros p; one_step p;eauto with proof. 
+(*
+{A, 1, 1, P & 1} ⊢ A ⊕ M
+*)
+Qed.
+Hint Resolve aux_342 : proof.
+Hint Rewrite aux_342 : proof.
+
+Lemma aux_344 : no_proof_for ({1, V ⊸ A, P & 1, (P ⊸ M) & 1, V}) M.
+Proof.
+  intros p; unusable_var_strong_tac 5%nat 6%nat p.
+Qed.
+Hint Resolve aux_344 : proof.
+
+Lemma aux_345 : all_proofs_of ({1, V ⊸ A, P & 1, (P ⊸ M) & 1, V}) (A ⊕ M).
+Proof.
+  intros p; one_step p;eauto with proof. 
+(*
+{A, 1, P & 1, (P ⊸ M) & 1} ⊢ A ⊕ M             +
+{A, 1, P & 1} ⊢ A ⊕ M                          +
+{V ⊸ A, P & 1, (P ⊸ M) & 1, V} ⊢ A ⊕ M        +
+{1, 1, V ⊸ A, P & 1, V} ⊢ A ⊕ M               +
+{1, V ⊸ A, P & 1, (P ⊸ M) & 1, V} ⊢ M         - e
+*)
+Qed.
+Hint Resolve aux_345 : proof.
+Hint Rewrite aux_345 : proof.
+
+Lemma aux_346 : all_proofs_of ({A, 1, P & 1, (E ⊸ A) & 1}) (A ⊕ M).
+Proof.
+  intros p; one_step p;eauto with proof. 
+Qed.
+Hint Resolve aux_346 : proof.
+Hint Rewrite aux_346 : proof.
+
+Lemma aux_347 : no_proof_for ({E ⊸ A, V ⊸ A, P & 1, V}) (A ⊕ M).
+Proof.
+  intros p; unusable_implies_tac 7%nat A p.
+Qed.
+Hint Resolve aux_347 : proof.
+
+Lemma aux_348 : all_proofs_of ({V ⊸ A, P & 1, (E ⊸ A) & 1, V}) (A ⊕ M).
+Proof.
+  intros p; one_step p;eauto with proof. 
+(*
+   {E ⊸ A, V ⊸ A, P & 1, V} ⊢ A ⊕ M    e
+*)
+Qed.
+Hint Resolve aux_348 : proof.
+Hint Rewrite aux_348 : proof.
+
+Lemma aux_353 : no_proof_for ({E ⊸ A, 1, V ⊸ A, P & 1, V}) (A ⊕ M).
+Proof.
+  intros p; unusable_implies_tac 7%nat A p.
+Qed.
+Hint Resolve aux_353 : proof.
+
+
+Lemma aux_349 : all_proofs_of ({1, V ⊸ A, P & 1, (E ⊸ A) & 1, V}) (A ⊕ M).
+Proof.
+  intros p; one_step p;eauto with proof. 
+(*
+{A, 1, P & 1, (E ⊸ A) & 1} ⊢ A ⊕ M                 +
+ {V ⊸ A, P & 1, (E ⊸ A) & 1, V} ⊢ A ⊕ M            +
+{E ⊸ A, 1, V ⊸ A, P & 1, V} ⊢ A ⊕ M                  - e
+
+*)
+Qed.
+Hint Resolve aux_349 : proof.
+Hint Rewrite aux_349 : proof.
+
+Lemma aux_350 : no_proof_for ({V ⊸ A, P & 1, (E ⊸ A) & 1, (P ⊸ M) & 1, V})  M.
+Proof.
+  intros p; unusable_var_strong_tac 5%nat 6%nat p.
+Qed.
+Hint Resolve aux_350 : proof.
+
+
+Lemma aux_112 : all_proofs_of ({V ⊸ A, P & 1, (E ⊸ A) & 1, (P ⊸ M) & 1, V}) (A ⊕ M).
+Proof.
+  intros p; one_step p;eauto with proof.
+(*
+{A, (P ⊸ M) & 1} ⊢ A ⊕ M                      +
+{A, (E ⊸ A) & 1, (P ⊸ M) & 1} ⊢ A ⊕ M           +
+{A, (E ⊸ A) & 1} ⊢ A ⊕ M                        + 
+{A, P & 1, (E ⊸ A) & 1, (P ⊸ M) & 1} ⊢ A ⊕ M    +
+{A, P & 1, (E ⊸ A) & 1} ⊢ A ⊕ M                  +
+{A, P & 1} ⊢ A ⊕ M                               +
+{A, P & 1, (P ⊸ M) & 1} ⊢ A ⊕ M                  +
+{E ⊸ A, V ⊸ A, P & 1, (P ⊸ M) & 1, V} ⊢ A ⊕ M   - e
+{P ⊸ M, V ⊸ A, P & 1, (E ⊸ A) & 1, V} ⊢ A ⊕ M   - 
+{1, V ⊸ A, (E ⊸ A) & 1, (P ⊸ M) & 1, V} ⊢ A ⊕ M +
+{1, V ⊸ A, P & 1, (P ⊸ M) & 1, V} ⊢ A ⊕ M       +
+{1, V ⊸ A, P & 1, (E ⊸ A) & 1, V} ⊢ A ⊕ M       +
+{V ⊸ A, P & 1, (E ⊸ A) & 1, (P ⊸ M) & 1, V} ⊢ M - e
+*)
+Qed.
+Hint Resolve aux_112 : proof.
+Hint Rewrite aux_112 : proof. 
+
+Lemma aux_351 : no_proof_for ({E ⊸ A, P & 1, (V ⊸ A) & 1, (P ⊸ M) & 1, V}) (A ⊕ M).
+Proof.
+  intros p; unusable_implies_tac 7%nat A p.
+Qed.
+Hint Resolve aux_351 : proof.
+
+Lemma aux_354 : no_proof_for ({P & 1, (V ⊸ A) & 1, (E ⊸ A) & 1, V}) P.
+Proof.
+  intros p; unusable_var_strong_tac 5%nat 6%nat p.
+Qed.
+Hint Resolve aux_354 : proof.
+
+Lemma aux_355 : no_proof_for ({P & 1, (V ⊸ A) & 1, V}) P.
+Proof.
+  intros p; unusable_var_strong_tac 5%nat 6%nat p.
+Qed.
+Hint Resolve aux_355 : proof.
+
+Lemma aux_356 : no_proof_for ({E ⊸ A, P ⊸ M, P & 1, (V ⊸ A) & 1, V}) (A ⊕ M).
+Proof.
+  intros p; unusable_implies_tac 7%nat A p.
+Qed.
+Hint Resolve aux_356 : proof.
+
+Lemma aux_357 : no_proof_for ({1, P ⊸ M, (V ⊸ A) & 1, (E ⊸ A) & 1, V}) (A ⊕ M).
+Proof.
+  intros p; unusable_implies_tac 1%nat M p.
+Qed.
+Hint Resolve aux_357 : proof.
+
+Lemma aux_358 : no_proof_for ({1, P ⊸ M, (V ⊸ A) & 1, (E ⊸ A) & 1, V}) (A ⊕ M).
+Proof.
+  intros p; unusable_implies_tac 1%nat M p.
+Qed.
+Hint Resolve aux_358 : proof.
+
+Lemma aux_359 : no_proof_for ({E ⊸ A, P ⊸ M, P & 1, (V ⊸ A) & 1, V}) A.
+Proof.
+  intros p; unusable_implies_tac 7%nat A p.
+Qed.
+Hint Resolve aux_359 : proof.
+
+Lemma aux_360 : no_proof_for ({1, P ⊸ M, (V ⊸ A) & 1, (E ⊸ A) & 1, V}) A.
+Proof.
+  intros p; unusable_implies_tac 1%nat M p.
+Qed.
+Hint Resolve aux_360 : proof.
+
+Lemma aux_361 : no_proof_for ({1, P ⊸ M, (V ⊸ A) & 1, V}) A.
+Proof.
+  intros p; unusable_implies_tac 1%nat M p.
+Qed.
+Hint Resolve aux_361 : proof.
+
+Lemma aux_362 : no_proof_for ({P ⊸ M, P & 1, (V ⊸ A) & 1, V}) A .
+Proof.
+  intros p;one_step p;eauto with proof.
+(*
+{1, P ⊸ M, (V ⊸ A) & 1, V} ⊢ A   e
+*)
+Qed.
+Hint Resolve aux_362 : proof.
+
+Lemma aux_363 : no_proof_for ({1, 1, P ⊸ M, (V ⊸ A) & 1, V}) A.
+Proof.
+  intros p; unusable_implies_tac 1%nat M p.
+Qed.
+Hint Resolve aux_363 : proof.
+
+Lemma aux_364 : no_proof_for ({1, P ⊸ M, P & 1, (V ⊸ A) & 1, V}) A.
+Proof.
+  intros p;one_step p;eauto with proof.
+(*
+{P ⊸ M, P & 1, (V ⊸ A) & 1, V} ⊢ A 
+{1, 1, P ⊸ M, (V ⊸ A) & 1, V} ⊢ A  
+*)
+Qed.
+Hint Resolve aux_364 : proof.
+
+Lemma aux_365 : no_proof_for ({P ⊸ M, P & 1, (V ⊸ A) & 1, (E ⊸ A) & 1, V}) A.
+Proof.
+  intros p;one_step p;eauto with proof.
+(*
+{E ⊸ A, P ⊸ M, P & 1, (V ⊸ A) & 1, V} ⊢ A     e
+{1, P ⊸ M, (V ⊸ A) & 1, (E ⊸ A) & 1, V} ⊢ A   e
+{1, P ⊸ M, P & 1, (V ⊸ A) & 1, V} ⊢ A         
+*)
+Qed.
+Hint Resolve aux_365 : proof.
+
+Lemma aux_366 : no_proof_for ({P ⊸ M, P & 1, (V ⊸ A) & 1, (E ⊸ A) & 1, V}) M.
+Proof.
+  intros p; unusable_var_strong_tac 5%nat 6%nat p.
+Qed.
+Hint Resolve aux_366 : proof. 
+
+Lemma aux_367 : no_proof_for ({1, P & 1, (V ⊸ A) & 1, V}) P.
+Proof.
+  intros p; unusable_var_strong_tac 5%nat 6%nat p.
+Qed.
+Hint Resolve aux_367 : proof. 
+
+Lemma aux_368 : no_proof_for({P ⊸ M, (V ⊸ A) & 1, V}) (A ⊕ M).
+Proof.
+  intros p; unusable_implies_tac 1%nat M p.
+Qed.
+Hint Resolve aux_368 : proof.
+
+Lemma aux_369 : no_proof_for ({1, P ⊸ M, (V ⊸ A) & 1, V}) M.
+Proof.
+  intros p; unusable_implies_tac 1%nat M p.
+Qed.
+Hint Resolve aux_369 : proof.
+
+Lemma aux_370 : no_proof_for ({1, P ⊸ M, (V ⊸ A) & 1, V}) (A ⊕ M).
+Proof.
+  intros p;one_step p;eauto with proof.
+(*
+{P ⊸ M, (V ⊸ A) & 1, V} ⊢ A ⊕ M  e
+{1, P ⊸ M, (V ⊸ A) & 1, V} ⊢ M   e
+*)
+Qed.
+Hint Resolve aux_370 : proof.
+
+Lemma aux_371 : no_proof_for ({P ⊸ M, P & 1, (V ⊸ A) & 1, V}) M. 
+Proof.
+  intros p; unusable_var_strong_tac 5%nat 6%nat p.
+Qed.
+Hint Resolve aux_371 : proof.
+
+Lemma aux_372 : no_proof_for ({P ⊸ M, P & 1, (V ⊸ A) & 1, V}) (A ⊕ M).
+Proof.
+  intros p;one_step p;eauto with proof.
+(*
+  {1, P ⊸ M, (V ⊸ A) & 1, V} ⊢ A ⊕ M
+   {P ⊸ M, P & 1, (V ⊸ A) & 1, V} ⊢ M         e
+*)
+Qed.
+Hint Resolve aux_372 : proof.
+
+Lemma aux_373 : no_proof_for ({1, 1, P ⊸ M, (V ⊸ A) & 1, V}) (A ⊕ M).
+Proof.
+  intros p; unusable_implies_tac 1%nat M p.
+Qed.
+Hint Resolve aux_373 : proof.
+
+Lemma aux_374 : no_proof_for ({1, P ⊸ M, P & 1, (V ⊸ A) & 1, V}) M.
+Proof.
+  intros p; unusable_var_strong_tac 5%nat 6%nat p.
+Qed.
+Hint Resolve aux_374 : proof.
+
+Lemma aux_375 : no_proof_for ({1, P ⊸ M, P & 1, (V ⊸ A) & 1, V}) (A ⊕ M).
+Proof.
+  intros p;one_step p;eauto with proof.
+(*
+{1, P & 1, (V ⊸ A) & 1, V} ⊢ P            e
+{P ⊸ M, P & 1, (V ⊸ A) & 1, V} ⊢ A ⊕ M    
+{1, 1, P ⊸ M, (V ⊸ A) & 1, V} ⊢ A ⊕ M    e
+{1, P ⊸ M, P & 1, (V ⊸ A) & 1, V} ⊢ M    e
+*)
+Qed.
+Hint Resolve aux_375 : proof.
+
+Lemma aux_376 : no_proof_for ({P ⊸ M, P & 1, (V ⊸ A) & 1, (E ⊸ A) & 1, V}) (A ⊕ M).
+Proof.
+  intros p;one_step p;eauto with proof.
+(*
+{P & 1, (V ⊸ A) & 1, (E ⊸ A) & 1, V} ⊢ P         e
+{P & 1, (V ⊸ A) & 1, V} ⊢ P                       e
+{E ⊸ A, P ⊸ M, P & 1, (V ⊸ A) & 1, V} ⊢ A ⊕ M    e
+{1, P ⊸ M, (V ⊸ A) & 1, (E ⊸ A) & 1, V} ⊢ A ⊕ M  e
+{1, P ⊸ M, (V ⊸ A) & 1, (E ⊸ A) & 1, V} ⊢ A ⊕ M  e
+{P ⊸ M, P & 1, (V ⊸ A) & 1, (E ⊸ A) & 1, V} ⊢ A   
+{P ⊸ M, P & 1, (V ⊸ A) & 1, (E ⊸ A) & 1, V} ⊢ M  e
+{1, P ⊸ M, P & 1, (V ⊸ A) & 1, V} ⊢ A ⊕ M
+*)
+Qed.
+Hint Resolve aux_376 : proof.
+
+Lemma aux_377 : all_proofs_of ({(V ⊸ A) & 1, (E ⊸ A) & 1, (P ⊸ M) & 1, V}) (A ⊕ M).
+Proof.
+  intros p;one_step p;eauto with proof.
+(*
+
+*)
+Qed.
+Hint Resolve proof_4 : proof.
+Hint Rewrite proof_4 : proof.
+
+Lemma aux_377 : all_proofs_of ({1, (V ⊸ A) & 1, (E ⊸ A) & 1, (P ⊸ M) & 1, V})  (A ⊕ M).
+Proof.
+  intros p;one_step p;eauto with proof.
+(*
+{(V ⊸ A) & 1, (E ⊸ A) & 1, (P ⊸ M) & 1, V} ⊢ A ⊕ M              +
+{E ⊸ A, 1, (V ⊸ A) & 1, (P ⊸ M) & 1, V} ⊢ A ⊕ M                 - e
+{1, 1, (V ⊸ A) & 1, (P ⊸ M) & 1, V} ⊢ A ⊕ M                     +
+{1, 1, (V ⊸ A) & 1, (E ⊸ A) & 1, V} ⊢ A ⊕ M                     +
+ {1, (V ⊸ A) & 1, (E ⊸ A) & 1, (P ⊸ M) & 1, V} ⊢ M              - e
+*)
+Qed.
+Hint Resolve proof_4 : proof.
+Hint Rewrite proof_4 : proof.
+
+
+Lemma proof_4 : all_proofs_of ({P&1,(V⊸A)&1,(E⊸A)&1,(P⊸M)&1,V}) (A⊕M).
+Proof.
+  intros p;one_step p;eauto with proof.
+(*
+{P, (V ⊸ A) & 1, (E ⊸ A) & 1, (P ⊸ M) & 1, V} ⊢ A ⊕ M    -
+{V ⊸ A, P & 1, (E ⊸ A) & 1, (P ⊸ M) & 1, V} ⊢ A ⊕ M      + 
+{E ⊸ A, P & 1, (V ⊸ A) & 1, (P ⊸ M) & 1, V} ⊢ A ⊕ M      e 
+{P ⊸ M, P & 1, (V ⊸ A) & 1, (E ⊸ A) & 1, V} ⊢ A ⊕ M      - 
+*{1, (V ⊸ A) & 1, (E ⊸ A) & 1, (P ⊸ M) & 1, V} ⊢ A ⊕ M    +
+{1, P & 1, (V ⊸ A) & 1, (P ⊸ M) & 1, V} ⊢ A ⊕ M           +
+{1, P & 1, (V ⊸ A) & 1, (E ⊸ A) & 1, V} ⊢ A ⊕ M          +
+{P & 1, (V ⊸ A) & 1, (E ⊸ A) & 1, (P ⊸ M) & 1, V} ⊢ M   +
+*)
+Qed.
+Hint Resolve proof_4 : proof.
+Hint Rewrite proof_4 : proof.
